{
  "exchanges": {
    "id": "ILCDex:63a79af11ab0467745a808dc6fc9d4ca_exchanges",
    "exchange": [
      {
        "id": "ILCDex:63a79af11ab0467745a808dc6fc9d4ca_exchanges_exchange_01",
        "dataSetInternalID": 0,
        "referenceToFlowDataSet": {
          "id": "ILCDex:63a79af11ab0467745a808dc6fc9d4ca_exchanges_exchange_01_referenceToFlowDataSet",
          "shortDescription": [
            {
              "id": "ILCDex:63a79af11ab0467745a808dc6fc9d4ca_exchanges_exchange_01_referenceToFlowDataSet_shortDescription_01",
              "value": " beForce Rck50 S5 XC3 D20 CEM II 42,5 R CAM20",
              "lang": "en"
            }
          ],
          "type": "flow data set",
          "refObjectId": "5e4009b3-9918-4d43-0fea-08dc6ff8f90b",
          "version": "00.01.000"
        },
        "meanAmount": 1.0,
        "referenceFlow": true,
        "resultingflowAmount": 1.0,
        "flowProperties": [
          {
            "id": "ILCDex:63a79af11ab0467745a808dc6fc9d4ca_exchanges_exchange_01_flowProperties_01",
            "referenceFlowProperty": true,
            "meanValue": 1.0,
            "referenceUnit": "m3",
            "unitGroupUUID": "93a60a57-a3c8-12da-a746-0800200c9a66",
            "nameFP": [
              {
                "id": "ILCDex:63a79af11ab0467745a808dc6fc9d4ca_exchanges_exchange_01_flowProperties_01_nameFP_01",
                "lang": "en",
                "value": "Volume"
              }
            ],
            "uuidFP": "93a60a56-a3c8-22da-a746-0800200c9a66"
          }
        ],
        "materialProperties": [
          {
            "id": "ILCDex:63a79af11ab0467745a808dc6fc9d4ca_exchanges_exchange_01_materialProperties_01",
            "name": "bulk density (kg/m^3)",
            "value": "2475.0",
            "unit": "bulk density (kg/m^3)",
            "unitDescription": "bulk density (kg/m^3)"
          },
          {
            "id": "ILCDex:63a79af11ab0467745a808dc6fc9d4ca_exchanges_exchange_01_materialProperties_02",
            "name": "compressive strength (mpa)",
            "value": "50.0",
            "unit": "Compressive strength (MPa)",
            "unitDescription": "Compressive strength (MPa)"
          }
        ],
        "typeOfFlow": "Product flow"
      },
      {
        "id": "ILCDex:63a79af11ab0467745a808dc6fc9d4ca_exchanges_exchange_02",
        "dataSetInternalID": 1,
        "referenceToFlowDataSet": {
          "id": "ILCDex:63a79af11ab0467745a808dc6fc9d4ca_exchanges_exchange_02_referenceToFlowDataSet",
          "shortDescription": [
            {
              "id": "ILCDex:63a79af11ab0467745a808dc6fc9d4ca_exchanges_exchange_02_referenceToFlowDataSet_shortDescription_01",
              "value": "Use of renewable primary energy as energy carrier (PERE)",
              "lang": "en"
            }
          ],
          "type": "flow data set",
          "refObjectId": "20f32be5-0398-4288-9b6d-accddd195317"
        },
        "meanAmount": 0.0,
        "resolvedFlowVersion": "35.00.000",
        "flowProperties": [],
        "typeOfFlow": "Other flow",
        "exchangeDirection": "INPUT",
        "otherEx": {
          "id": "ILCDex:63a79af11ab0467745a808dc6fc9d4ca_exchanges_exchange_02_otherEx",
          "anies": [
            {
              "id": "ILCDex:63a79af11ab0467745a808dc6fc9d4ca_exchanges_exchange_02_otherEx_anies_moduleA1",
              "value": "200.331850129794",
              "module": "A1"
            },
            {
              "id": "ILCDex:63a79af11ab0467745a808dc6fc9d4ca_exchanges_exchange_02_otherEx_anies_moduleA2",
              "value": "2.48154315611149",
              "module": "A2"
            },
            {
              "id": "ILCDex:63a79af11ab0467745a808dc6fc9d4ca_exchanges_exchange_02_otherEx_anies_moduleA3",
              "value": "1.10198021926091",
              "module": "A3"
            },
            {
              "id": "ILCDex:63a79af11ab0467745a808dc6fc9d4ca_exchanges_exchange_02_otherEx_anies_moduleA1A3",
              "value": "203.915373505166",
              "module": "A1-A3"
            },
            {
              "id": "ILCDex:63a79af11ab0467745a808dc6fc9d4ca_exchanges_exchange_02_otherEx_anies_moduleA4",
              "value": "ND",
              "module": "A4"
            },
            {
              "id": "ILCDex:63a79af11ab0467745a808dc6fc9d4ca_exchanges_exchange_02_otherEx_anies_moduleA5",
              "value": "ND",
              "module": "A5"
            },
            {
              "id": "ILCDex:63a79af11ab0467745a808dc6fc9d4ca_exchanges_exchange_02_otherEx_anies_moduleB1",
              "value": "0",
              "module": "B1"
            },
            {
              "id": "ILCDex:63a79af11ab0467745a808dc6fc9d4ca_exchanges_exchange_02_otherEx_anies_moduleB2",
              "value": "0",
              "module": "B2"
            },
            {
              "id": "ILCDex:63a79af11ab0467745a808dc6fc9d4ca_exchanges_exchange_02_otherEx_anies_moduleB3",
              "value": "0",
              "module": "B3"
            },
            {
              "id": "ILCDex:63a79af11ab0467745a808dc6fc9d4ca_exchanges_exchange_02_otherEx_anies_moduleB4",
              "value": "0",
              "module": "B4"
            },
            {
              "id": "ILCDex:63a79af11ab0467745a808dc6fc9d4ca_exchanges_exchange_02_otherEx_anies_moduleB5",
              "value": "0",
              "module": "B5"
            },
            {
              "id": "ILCDex:63a79af11ab0467745a808dc6fc9d4ca_exchanges_exchange_02_otherEx_anies_moduleB6",
              "value": "0",
              "module": "B6"
            },
            {
              "id": "ILCDex:63a79af11ab0467745a808dc6fc9d4ca_exchanges_exchange_02_otherEx_anies_moduleB7",
              "value": "0",
              "module": "B7"
            },
            {
              "id": "ILCDex:63a79af11ab0467745a808dc6fc9d4ca_exchanges_exchange_02_otherEx_anies_moduleC1",
              "value": "0.758557945488",
              "module": "C1"
            },
            {
              "id": "ILCDex:63a79af11ab0467745a808dc6fc9d4ca_exchanges_exchange_02_otherEx_anies_moduleC2",
              "value": "3.542532703875",
              "module": "C2"
            },
            {
              "id": "ILCDex:63a79af11ab0467745a808dc6fc9d4ca_exchanges_exchange_02_otherEx_anies_moduleC3",
              "value": "8.991775066725",
              "module": "C3"
            },
            {
              "id": "ILCDex:63a79af11ab0467745a808dc6fc9d4ca_exchanges_exchange_02_otherEx_anies_moduleC4",
              "value": "1.953996895125",
              "module": "C4"
            },
            {
              "id": "ILCDex:63a79af11ab0467745a808dc6fc9d4ca_exchanges_exchange_02_otherEx_anies_moduleD",
              "value": "-14.21955172935",
              "module": "D"
            },
            {
              "id": "ILCDex:63a79af11ab0467745a808dc6fc9d4ca_exchanges_exchange_02_otherEx_anies_19",
              "name": "referenceToUnitGroupDataSet",
              "objectValue": {
                "id": "ILCDex:63a79af11ab0467745a808dc6fc9d4ca_exchanges_exchange_02_otherEx_anies_19_objectValue",
                "shortDescription": [
                  {
                    "id": "ILCDex:63a79af11ab0467745a808dc6fc9d4ca_exchanges_exchange_02_otherEx_anies_19_objectValue_shortDescription_01",
                    "value": "MJ"
                  }
                ],
                "type": "unit group data set",
                "refObjectId": "93a60a57-a3c8-11da-a746-0800200c9a66",
                "refObjectUri": "../unitgroups/93a60a57-a3c8-11da-a746-0800200c9a66"
              }
            }
          ]
        },
        "classificationEx": {
          "id": "ILCDex:63a79af11ab0467745a808dc6fc9d4ca_exchanges_exchange_02_classificationEx",
          "classHierarchy": "Quantities",
          "nameClass": "GaBiCategories"
        }
      },
      {
        "id": "ILCDex:63a79af11ab0467745a808dc6fc9d4ca_exchanges_exchange_03",
        "dataSetInternalID": 2,
        "referenceToFlowDataSet": {
          "id": "ILCDex:63a79af11ab0467745a808dc6fc9d4ca_exchanges_exchange_03_referenceToFlowDataSet",
          "shortDescription": [
            {
              "id": "ILCDex:63a79af11ab0467745a808dc6fc9d4ca_exchanges_exchange_03_referenceToFlowDataSet_shortDescription_01",
              "value": "Use of renewable primary energy resources used as raw materials (PERM)",
              "lang": "en"
            }
          ],
          "type": "flow data set",
          "refObjectId": "fb3ec0de-548d-4508-aea5-00b73bf6f702"
        },
        "meanAmount": 0.0,
        "resolvedFlowVersion": "35.00.000",
        "flowProperties": [],
        "typeOfFlow": "Other flow",
        "exchangeDirection": "INPUT",
        "otherEx": {
          "id": "ILCDex:63a79af11ab0467745a808dc6fc9d4ca_exchanges_exchange_03_otherEx",
          "anies": [
            {
              "id": "ILCDex:63a79af11ab0467745a808dc6fc9d4ca_exchanges_exchange_03_otherEx_anies_moduleA1",
              "value": "0",
              "module": "A1"
            },
            {
              "id": "ILCDex:63a79af11ab0467745a808dc6fc9d4ca_exchanges_exchange_03_otherEx_anies_moduleA2",
              "value": "0",
              "module": "A2"
            },
            {
              "id": "ILCDex:63a79af11ab0467745a808dc6fc9d4ca_exchanges_exchange_03_otherEx_anies_moduleA3",
              "value": "0",
              "module": "A3"
            },
            {
              "id": "ILCDex:63a79af11ab0467745a808dc6fc9d4ca_exchanges_exchange_03_otherEx_anies_moduleA1A3",
              "value": "0",
              "module": "A1-A3"
            },
            {
              "id": "ILCDex:63a79af11ab0467745a808dc6fc9d4ca_exchanges_exchange_03_otherEx_anies_moduleA4",
              "value": "ND",
              "module": "A4"
            },
            {
              "id": "ILCDex:63a79af11ab0467745a808dc6fc9d4ca_exchanges_exchange_03_otherEx_anies_moduleA5",
              "value": "ND",
              "module": "A5"
            },
            {
              "id": "ILCDex:63a79af11ab0467745a808dc6fc9d4ca_exchanges_exchange_03_otherEx_anies_moduleB1",
              "value": "0",
              "module": "B1"
            },
            {
              "id": "ILCDex:63a79af11ab0467745a808dc6fc9d4ca_exchanges_exchange_03_otherEx_anies_moduleB2",
              "value": "0",
              "module": "B2"
            },
            {
              "id": "ILCDex:63a79af11ab0467745a808dc6fc9d4ca_exchanges_exchange_03_otherEx_anies_moduleB3",
              "value": "0",
              "module": "B3"
            },
            {
              "id": "ILCDex:63a79af11ab0467745a808dc6fc9d4ca_exchanges_exchange_03_otherEx_anies_moduleB4",
              "value": "0",
              "module": "B4"
            },
            {
              "id": "ILCDex:63a79af11ab0467745a808dc6fc9d4ca_exchanges_exchange_03_otherEx_anies_moduleB5",
              "value": "0",
              "module": "B5"
            },
            {
              "id": "ILCDex:63a79af11ab0467745a808dc6fc9d4ca_exchanges_exchange_03_otherEx_anies_moduleB6",
              "value": "0",
              "module": "B6"
            },
            {
              "id": "ILCDex:63a79af11ab0467745a808dc6fc9d4ca_exchanges_exchange_03_otherEx_anies_moduleB7",
              "value": "0",
              "module": "B7"
            },
            {
              "id": "ILCDex:63a79af11ab0467745a808dc6fc9d4ca_exchanges_exchange_03_otherEx_anies_moduleC1",
              "value": "0",
              "module": "C1"
            },
            {
              "id": "ILCDex:63a79af11ab0467745a808dc6fc9d4ca_exchanges_exchange_03_otherEx_anies_moduleC2",
              "value": "0",
              "module": "C2"
            },
            {
              "id": "ILCDex:63a79af11ab0467745a808dc6fc9d4ca_exchanges_exchange_03_otherEx_anies_moduleC3",
              "value": "0",
              "module": "C3"
            },
            {
              "id": "ILCDex:63a79af11ab0467745a808dc6fc9d4ca_exchanges_exchange_03_otherEx_anies_moduleC4",
              "value": "0",
              "module": "C4"
            },
            {
              "id": "ILCDex:63a79af11ab0467745a808dc6fc9d4ca_exchanges_exchange_03_otherEx_anies_moduleD",
              "value": "0",
              "module": "D"
            },
            {
              "id": "ILCDex:63a79af11ab0467745a808dc6fc9d4ca_exchanges_exchange_03_otherEx_anies_19",
              "name": "referenceToUnitGroupDataSet",
              "objectValue": {
                "id": "ILCDex:63a79af11ab0467745a808dc6fc9d4ca_exchanges_exchange_03_otherEx_anies_19_objectValue",
                "shortDescription": [
                  {
                    "id": "ILCDex:63a79af11ab0467745a808dc6fc9d4ca_exchanges_exchange_03_otherEx_anies_19_objectValue_shortDescription_01",
                    "value": "MJ"
                  }
                ],
                "type": "unit group data set",
                "refObjectId": "93a60a57-a3c8-11da-a746-0800200c9a66",
                "refObjectUri": "../unitgroups/93a60a57-a3c8-11da-a746-0800200c9a66"
              }
            }
          ]
        },
        "classificationEx": {
          "id": "ILCDex:63a79af11ab0467745a808dc6fc9d4ca_exchanges_exchange_03_classificationEx",
          "classHierarchy": "Quantities",
          "nameClass": "GaBiCategories"
        }
      },
      {
        "id": "ILCDex:63a79af11ab0467745a808dc6fc9d4ca_exchanges_exchange_04",
        "dataSetInternalID": 3,
        "referenceToFlowDataSet": {
          "id": "ILCDex:63a79af11ab0467745a808dc6fc9d4ca_exchanges_exchange_04_referenceToFlowDataSet",
          "shortDescription": [
            {
              "id": "ILCDex:63a79af11ab0467745a808dc6fc9d4ca_exchanges_exchange_04_referenceToFlowDataSet_shortDescription_01",
              "value": "Total use of renewable primary energy (PERT)",
              "lang": "en"
            }
          ],
          "type": "flow data set",
          "refObjectId": "53f97275-fa8a-4cdd-9024-65936002acd0"
        },
        "meanAmount": 0.0,
        "resolvedFlowVersion": "35.00.000",
        "flowProperties": [],
        "typeOfFlow": "Other flow",
        "exchangeDirection": "INPUT",
        "otherEx": {
          "id": "ILCDex:63a79af11ab0467745a808dc6fc9d4ca_exchanges_exchange_04_otherEx",
          "anies": [
            {
              "id": "ILCDex:63a79af11ab0467745a808dc6fc9d4ca_exchanges_exchange_04_otherEx_anies_moduleA1",
              "value": "200.331850129794",
              "module": "A1"
            },
            {
              "id": "ILCDex:63a79af11ab0467745a808dc6fc9d4ca_exchanges_exchange_04_otherEx_anies_moduleA2",
              "value": "2.48154315611149",
              "module": "A2"
            },
            {
              "id": "ILCDex:63a79af11ab0467745a808dc6fc9d4ca_exchanges_exchange_04_otherEx_anies_moduleA3",
              "value": "1.10198021926091",
              "module": "A3"
            },
            {
              "id": "ILCDex:63a79af11ab0467745a808dc6fc9d4ca_exchanges_exchange_04_otherEx_anies_moduleA1A3",
              "value": "203.915373505166",
              "module": "A1-A3"
            },
            {
              "id": "ILCDex:63a79af11ab0467745a808dc6fc9d4ca_exchanges_exchange_04_otherEx_anies_moduleA4",
              "value": "ND",
              "module": "A4"
            },
            {
              "id": "ILCDex:63a79af11ab0467745a808dc6fc9d4ca_exchanges_exchange_04_otherEx_anies_moduleA5",
              "value": "ND",
              "module": "A5"
            },
            {
              "id": "ILCDex:63a79af11ab0467745a808dc6fc9d4ca_exchanges_exchange_04_otherEx_anies_moduleB1",
              "value": "0",
              "module": "B1"
            },
            {
              "id": "ILCDex:63a79af11ab0467745a808dc6fc9d4ca_exchanges_exchange_04_otherEx_anies_moduleB2",
              "value": "0",
              "module": "B2"
            },
            {
              "id": "ILCDex:63a79af11ab0467745a808dc6fc9d4ca_exchanges_exchange_04_otherEx_anies_moduleB3",
              "value": "0",
              "module": "B3"
            },
            {
              "id": "ILCDex:63a79af11ab0467745a808dc6fc9d4ca_exchanges_exchange_04_otherEx_anies_moduleB4",
              "value": "0",
              "module": "B4"
            },
            {
              "id": "ILCDex:63a79af11ab0467745a808dc6fc9d4ca_exchanges_exchange_04_otherEx_anies_moduleB5",
              "value": "0",
              "module": "B5"
            },
            {
              "id": "ILCDex:63a79af11ab0467745a808dc6fc9d4ca_exchanges_exchange_04_otherEx_anies_moduleB6",
              "value": "0",
              "module": "B6"
            },
            {
              "id": "ILCDex:63a79af11ab0467745a808dc6fc9d4ca_exchanges_exchange_04_otherEx_anies_moduleB7",
              "value": "0",
              "module": "B7"
            },
            {
              "id": "ILCDex:63a79af11ab0467745a808dc6fc9d4ca_exchanges_exchange_04_otherEx_anies_moduleC1",
              "value": "0.758557945488",
              "module": "C1"
            },
            {
              "id": "ILCDex:63a79af11ab0467745a808dc6fc9d4ca_exchanges_exchange_04_otherEx_anies_moduleC2",
              "value": "3.542532703875",
              "module": "C2"
            },
            {
              "id": "ILCDex:63a79af11ab0467745a808dc6fc9d4ca_exchanges_exchange_04_otherEx_anies_moduleC3",
              "value": "8.991775066725",
              "module": "C3"
            },
            {
              "id": "ILCDex:63a79af11ab0467745a808dc6fc9d4ca_exchanges_exchange_04_otherEx_anies_moduleC4",
              "value": "1.953996895125",
              "module": "C4"
            },
            {
              "id": "ILCDex:63a79af11ab0467745a808dc6fc9d4ca_exchanges_exchange_04_otherEx_anies_moduleD",
              "value": "-14.21955172935",
              "module": "D"
            },
            {
              "id": "ILCDex:63a79af11ab0467745a808dc6fc9d4ca_exchanges_exchange_04_otherEx_anies_19",
              "name": "referenceToUnitGroupDataSet",
              "objectValue": {
                "id": "ILCDex:63a79af11ab0467745a808dc6fc9d4ca_exchanges_exchange_04_otherEx_anies_19_objectValue",
                "shortDescription": [
                  {
                    "id": "ILCDex:63a79af11ab0467745a808dc6fc9d4ca_exchanges_exchange_04_otherEx_anies_19_objectValue_shortDescription_01",
                    "value": "MJ"
                  }
                ],
                "type": "unit group data set",
                "refObjectId": "93a60a57-a3c8-11da-a746-0800200c9a66",
                "refObjectUri": "../unitgroups/93a60a57-a3c8-11da-a746-0800200c9a66"
              }
            }
          ]
        },
        "classificationEx": {
          "id": "ILCDex:63a79af11ab0467745a808dc6fc9d4ca_exchanges_exchange_04_classificationEx",
          "classHierarchy": "Quantities / Environmental quantities / EPD EN 15804 / LCI indicators",
          "nameClass": "GaBiCategories"
        }
      },
      {
        "id": "ILCDex:63a79af11ab0467745a808dc6fc9d4ca_exchanges_exchange_05",
        "dataSetInternalID": 4,
        "referenceToFlowDataSet": {
          "id": "ILCDex:63a79af11ab0467745a808dc6fc9d4ca_exchanges_exchange_05_referenceToFlowDataSet",
          "shortDescription": [
            {
              "id": "ILCDex:63a79af11ab0467745a808dc6fc9d4ca_exchanges_exchange_05_referenceToFlowDataSet_shortDescription_01",
              "value": "Use of non renewable primary energy as energy carrier (PENRE)",
              "lang": "en"
            }
          ],
          "type": "flow data set",
          "refObjectId": "ac857178-2b45-46ec-892a-a9a4332f0372"
        },
        "meanAmount": 0.0,
        "resolvedFlowVersion": "35.00.000",
        "flowProperties": [],
        "typeOfFlow": "Other flow",
        "exchangeDirection": "INPUT",
        "otherEx": {
          "id": "ILCDex:63a79af11ab0467745a808dc6fc9d4ca_exchanges_exchange_05_otherEx",
          "anies": [
            {
              "id": "ILCDex:63a79af11ab0467745a808dc6fc9d4ca_exchanges_exchange_05_otherEx_anies_moduleA1",
              "value": "2282.2299545615",
              "module": "A1"
            },
            {
              "id": "ILCDex:63a79af11ab0467745a808dc6fc9d4ca_exchanges_exchange_05_otherEx_anies_moduleA2",
              "value": "173.485372713409",
              "module": "A2"
            },
            {
              "id": "ILCDex:63a79af11ab0467745a808dc6fc9d4ca_exchanges_exchange_05_otherEx_anies_moduleA3",
              "value": "17.736093614435",
              "module": "A3"
            },
            {
              "id": "ILCDex:63a79af11ab0467745a808dc6fc9d4ca_exchanges_exchange_05_otherEx_anies_moduleA1A3",
              "value": "2473.45142088935",
              "module": "A1-A3"
            },
            {
              "id": "ILCDex:63a79af11ab0467745a808dc6fc9d4ca_exchanges_exchange_05_otherEx_anies_moduleA4",
              "value": "ND",
              "module": "A4"
            },
            {
              "id": "ILCDex:63a79af11ab0467745a808dc6fc9d4ca_exchanges_exchange_05_otherEx_anies_moduleA5",
              "value": "ND",
              "module": "A5"
            },
            {
              "id": "ILCDex:63a79af11ab0467745a808dc6fc9d4ca_exchanges_exchange_05_otherEx_anies_moduleB1",
              "value": "0",
              "module": "B1"
            },
            {
              "id": "ILCDex:63a79af11ab0467745a808dc6fc9d4ca_exchanges_exchange_05_otherEx_anies_moduleB2",
              "value": "0",
              "module": "B2"
            },
            {
              "id": "ILCDex:63a79af11ab0467745a808dc6fc9d4ca_exchanges_exchange_05_otherEx_anies_moduleB3",
              "value": "0",
              "module": "B3"
            },
            {
              "id": "ILCDex:63a79af11ab0467745a808dc6fc9d4ca_exchanges_exchange_05_otherEx_anies_moduleB4",
              "value": "0",
              "module": "B4"
            },
            {
              "id": "ILCDex:63a79af11ab0467745a808dc6fc9d4ca_exchanges_exchange_05_otherEx_anies_moduleB5",
              "value": "0",
              "module": "B5"
            },
            {
              "id": "ILCDex:63a79af11ab0467745a808dc6fc9d4ca_exchanges_exchange_05_otherEx_anies_moduleB6",
              "value": "0",
              "module": "B6"
            },
            {
              "id": "ILCDex:63a79af11ab0467745a808dc6fc9d4ca_exchanges_exchange_05_otherEx_anies_moduleB7",
              "value": "0",
              "module": "B7"
            },
            {
              "id": "ILCDex:63a79af11ab0467745a808dc6fc9d4ca_exchanges_exchange_05_otherEx_anies_moduleC1",
              "value": "129.71448565334",
              "module": "C1"
            },
            {
              "id": "ILCDex:63a79af11ab0467745a808dc6fc9d4ca_exchanges_exchange_05_otherEx_anies_moduleC2",
              "value": "141.28759041705",
              "module": "C2"
            },
            {
              "id": "ILCDex:63a79af11ab0467745a808dc6fc9d4ca_exchanges_exchange_05_otherEx_anies_moduleC3",
              "value": "82.261703816325",
              "module": "C3"
            },
            {
              "id": "ILCDex:63a79af11ab0467745a808dc6fc9d4ca_exchanges_exchange_05_otherEx_anies_moduleC4",
              "value": "75.238478050725",
              "module": "C4"
            },
            {
              "id": "ILCDex:63a79af11ab0467745a808dc6fc9d4ca_exchanges_exchange_05_otherEx_anies_moduleD",
              "value": "-173.534940045225",
              "module": "D"
            },
            {
              "id": "ILCDex:63a79af11ab0467745a808dc6fc9d4ca_exchanges_exchange_05_otherEx_anies_19",
              "name": "referenceToUnitGroupDataSet",
              "objectValue": {
                "id": "ILCDex:63a79af11ab0467745a808dc6fc9d4ca_exchanges_exchange_05_otherEx_anies_19_objectValue",
                "shortDescription": [
                  {
                    "id": "ILCDex:63a79af11ab0467745a808dc6fc9d4ca_exchanges_exchange_05_otherEx_anies_19_objectValue_shortDescription_01",
                    "value": "MJ"
                  }
                ],
                "type": "unit group data set",
                "refObjectId": "93a60a57-a3c8-11da-a746-0800200c9a66",
                "refObjectUri": "../unitgroups/93a60a57-a3c8-11da-a746-0800200c9a66"
              }
            }
          ]
        },
        "classificationEx": {
          "id": "ILCDex:63a79af11ab0467745a808dc6fc9d4ca_exchanges_exchange_05_classificationEx",
          "classHierarchy": "Quantities",
          "nameClass": "GaBiCategories"
        }
      },
      {
        "id": "ILCDex:63a79af11ab0467745a808dc6fc9d4ca_exchanges_exchange_06",
        "dataSetInternalID": 5,
        "referenceToFlowDataSet": {
          "id": "ILCDex:63a79af11ab0467745a808dc6fc9d4ca_exchanges_exchange_06_referenceToFlowDataSet",
          "shortDescription": [
            {
              "id": "ILCDex:63a79af11ab0467745a808dc6fc9d4ca_exchanges_exchange_06_referenceToFlowDataSet_shortDescription_01",
              "value": "Use of non renewable primary energy resources used as raw materials (PENRM)",
              "lang": "en"
            }
          ],
          "type": "flow data set",
          "refObjectId": "1421caa0-679d-4bf4-b282-0eb850ccae27"
        },
        "meanAmount": 0.0,
        "resolvedFlowVersion": "35.00.000",
        "flowProperties": [],
        "typeOfFlow": "Other flow",
        "exchangeDirection": "INPUT",
        "otherEx": {
          "id": "ILCDex:63a79af11ab0467745a808dc6fc9d4ca_exchanges_exchange_06_otherEx",
          "anies": [
            {
              "id": "ILCDex:63a79af11ab0467745a808dc6fc9d4ca_exchanges_exchange_06_otherEx_anies_moduleA1",
              "value": "0.00865",
              "module": "A1"
            },
            {
              "id": "ILCDex:63a79af11ab0467745a808dc6fc9d4ca_exchanges_exchange_06_otherEx_anies_moduleA2",
              "value": "0",
              "module": "A2"
            },
            {
              "id": "ILCDex:63a79af11ab0467745a808dc6fc9d4ca_exchanges_exchange_06_otherEx_anies_moduleA3",
              "value": "0",
              "module": "A3"
            },
            {
              "id": "ILCDex:63a79af11ab0467745a808dc6fc9d4ca_exchanges_exchange_06_otherEx_anies_moduleA1A3",
              "value": "0.00865",
              "module": "A1-A3"
            },
            {
              "id": "ILCDex:63a79af11ab0467745a808dc6fc9d4ca_exchanges_exchange_06_otherEx_anies_moduleA4",
              "value": "ND",
              "module": "A4"
            },
            {
              "id": "ILCDex:63a79af11ab0467745a808dc6fc9d4ca_exchanges_exchange_06_otherEx_anies_moduleA5",
              "value": "ND",
              "module": "A5"
            },
            {
              "id": "ILCDex:63a79af11ab0467745a808dc6fc9d4ca_exchanges_exchange_06_otherEx_anies_moduleB1",
              "value": "0",
              "module": "B1"
            },
            {
              "id": "ILCDex:63a79af11ab0467745a808dc6fc9d4ca_exchanges_exchange_06_otherEx_anies_moduleB2",
              "value": "0",
              "module": "B2"
            },
            {
              "id": "ILCDex:63a79af11ab0467745a808dc6fc9d4ca_exchanges_exchange_06_otherEx_anies_moduleB3",
              "value": "0",
              "module": "B3"
            },
            {
              "id": "ILCDex:63a79af11ab0467745a808dc6fc9d4ca_exchanges_exchange_06_otherEx_anies_moduleB4",
              "value": "0",
              "module": "B4"
            },
            {
              "id": "ILCDex:63a79af11ab0467745a808dc6fc9d4ca_exchanges_exchange_06_otherEx_anies_moduleB5",
              "value": "0",
              "module": "B5"
            },
            {
              "id": "ILCDex:63a79af11ab0467745a808dc6fc9d4ca_exchanges_exchange_06_otherEx_anies_moduleB6",
              "value": "0",
              "module": "B6"
            },
            {
              "id": "ILCDex:63a79af11ab0467745a808dc6fc9d4ca_exchanges_exchange_06_otherEx_anies_moduleB7",
              "value": "0",
              "module": "B7"
            },
            {
              "id": "ILCDex:63a79af11ab0467745a808dc6fc9d4ca_exchanges_exchange_06_otherEx_anies_moduleC1",
              "value": "0",
              "module": "C1"
            },
            {
              "id": "ILCDex:63a79af11ab0467745a808dc6fc9d4ca_exchanges_exchange_06_otherEx_anies_moduleC2",
              "value": "0",
              "module": "C2"
            },
            {
              "id": "ILCDex:63a79af11ab0467745a808dc6fc9d4ca_exchanges_exchange_06_otherEx_anies_moduleC3",
              "value": "0",
              "module": "C3"
            },
            {
              "id": "ILCDex:63a79af11ab0467745a808dc6fc9d4ca_exchanges_exchange_06_otherEx_anies_moduleC4",
              "value": "0",
              "module": "C4"
            },
            {
              "id": "ILCDex:63a79af11ab0467745a808dc6fc9d4ca_exchanges_exchange_06_otherEx_anies_moduleD",
              "value": "0",
              "module": "D"
            },
            {
              "id": "ILCDex:63a79af11ab0467745a808dc6fc9d4ca_exchanges_exchange_06_otherEx_anies_19",
              "name": "referenceToUnitGroupDataSet",
              "objectValue": {
                "id": "ILCDex:63a79af11ab0467745a808dc6fc9d4ca_exchanges_exchange_06_otherEx_anies_19_objectValue",
                "shortDescription": [
                  {
                    "id": "ILCDex:63a79af11ab0467745a808dc6fc9d4ca_exchanges_exchange_06_otherEx_anies_19_objectValue_shortDescription_01",
                    "value": "MJ"
                  }
                ],
                "type": "unit group data set",
                "refObjectId": "93a60a57-a3c8-11da-a746-0800200c9a66",
                "refObjectUri": "../unitgroups/93a60a57-a3c8-11da-a746-0800200c9a66"
              }
            }
          ]
        },
        "classificationEx": {
          "id": "ILCDex:63a79af11ab0467745a808dc6fc9d4ca_exchanges_exchange_06_classificationEx",
          "classHierarchy": "Quantities",
          "nameClass": "GaBiCategories"
        }
      },
      {
        "id": "ILCDex:63a79af11ab0467745a808dc6fc9d4ca_exchanges_exchange_07",
        "dataSetInternalID": 6,
        "referenceToFlowDataSet": {
          "id": "ILCDex:63a79af11ab0467745a808dc6fc9d4ca_exchanges_exchange_07_referenceToFlowDataSet",
          "shortDescription": [
            {
              "id": "ILCDex:63a79af11ab0467745a808dc6fc9d4ca_exchanges_exchange_07_referenceToFlowDataSet_shortDescription_01",
              "value": "Total use of non renewable primary energy resource (PENRT)",
              "lang": "en"
            }
          ],
          "type": "flow data set",
          "refObjectId": "06159210-646b-4c8d-8583-da9b3b95a6c1"
        },
        "meanAmount": 0.0,
        "resolvedFlowVersion": "35.00.000",
        "flowProperties": [],
        "typeOfFlow": "Other flow",
        "exchangeDirection": "INPUT",
        "otherEx": {
          "id": "ILCDex:63a79af11ab0467745a808dc6fc9d4ca_exchanges_exchange_07_otherEx",
          "anies": [
            {
              "id": "ILCDex:63a79af11ab0467745a808dc6fc9d4ca_exchanges_exchange_07_otherEx_anies_moduleA1",
              "value": "2282.2386045615",
              "module": "A1"
            },
            {
              "id": "ILCDex:63a79af11ab0467745a808dc6fc9d4ca_exchanges_exchange_07_otherEx_anies_moduleA2",
              "value": "173.485372713409",
              "module": "A2"
            },
            {
              "id": "ILCDex:63a79af11ab0467745a808dc6fc9d4ca_exchanges_exchange_07_otherEx_anies_moduleA3",
              "value": "17.736093614435",
              "module": "A3"
            },
            {
              "id": "ILCDex:63a79af11ab0467745a808dc6fc9d4ca_exchanges_exchange_07_otherEx_anies_moduleA1A3",
              "value": "2473.46007088935",
              "module": "A1-A3"
            },
            {
              "id": "ILCDex:63a79af11ab0467745a808dc6fc9d4ca_exchanges_exchange_07_otherEx_anies_moduleA4",
              "value": "ND",
              "module": "A4"
            },
            {
              "id": "ILCDex:63a79af11ab0467745a808dc6fc9d4ca_exchanges_exchange_07_otherEx_anies_moduleA5",
              "value": "ND",
              "module": "A5"
            },
            {
              "id": "ILCDex:63a79af11ab0467745a808dc6fc9d4ca_exchanges_exchange_07_otherEx_anies_moduleB1",
              "value": "0",
              "module": "B1"
            },
            {
              "id": "ILCDex:63a79af11ab0467745a808dc6fc9d4ca_exchanges_exchange_07_otherEx_anies_moduleB2",
              "value": "0",
              "module": "B2"
            },
            {
              "id": "ILCDex:63a79af11ab0467745a808dc6fc9d4ca_exchanges_exchange_07_otherEx_anies_moduleB3",
              "value": "0",
              "module": "B3"
            },
            {
              "id": "ILCDex:63a79af11ab0467745a808dc6fc9d4ca_exchanges_exchange_07_otherEx_anies_moduleB4",
              "value": "0",
              "module": "B4"
            },
            {
              "id": "ILCDex:63a79af11ab0467745a808dc6fc9d4ca_exchanges_exchange_07_otherEx_anies_moduleB5",
              "value": "0",
              "module": "B5"
            },
            {
              "id": "ILCDex:63a79af11ab0467745a808dc6fc9d4ca_exchanges_exchange_07_otherEx_anies_moduleB6",
              "value": "0",
              "module": "B6"
            },
            {
              "id": "ILCDex:63a79af11ab0467745a808dc6fc9d4ca_exchanges_exchange_07_otherEx_anies_moduleB7",
              "value": "0",
              "module": "B7"
            },
            {
              "id": "ILCDex:63a79af11ab0467745a808dc6fc9d4ca_exchanges_exchange_07_otherEx_anies_moduleC1",
              "value": "129.71448565334",
              "module": "C1"
            },
            {
              "id": "ILCDex:63a79af11ab0467745a808dc6fc9d4ca_exchanges_exchange_07_otherEx_anies_moduleC2",
              "value": "141.28759041705",
              "module": "C2"
            },
            {
              "id": "ILCDex:63a79af11ab0467745a808dc6fc9d4ca_exchanges_exchange_07_otherEx_anies_moduleC3",
              "value": "82.261703816325",
              "module": "C3"
            },
            {
              "id": "ILCDex:63a79af11ab0467745a808dc6fc9d4ca_exchanges_exchange_07_otherEx_anies_moduleC4",
              "value": "75.238478050725",
              "module": "C4"
            },
            {
              "id": "ILCDex:63a79af11ab0467745a808dc6fc9d4ca_exchanges_exchange_07_otherEx_anies_moduleD",
              "value": "-173.534940045225",
              "module": "D"
            },
            {
              "id": "ILCDex:63a79af11ab0467745a808dc6fc9d4ca_exchanges_exchange_07_otherEx_anies_19",
              "name": "referenceToUnitGroupDataSet",
              "objectValue": {
                "id": "ILCDex:63a79af11ab0467745a808dc6fc9d4ca_exchanges_exchange_07_otherEx_anies_19_objectValue",
                "shortDescription": [
                  {
                    "id": "ILCDex:63a79af11ab0467745a808dc6fc9d4ca_exchanges_exchange_07_otherEx_anies_19_objectValue_shortDescription_01",
                    "value": "MJ"
                  }
                ],
                "type": "unit group data set",
                "refObjectId": "93a60a57-a3c8-11da-a746-0800200c9a66",
                "refObjectUri": "../unitgroups/93a60a57-a3c8-11da-a746-0800200c9a66"
              }
            }
          ]
        },
        "classificationEx": {
          "id": "ILCDex:63a79af11ab0467745a808dc6fc9d4ca_exchanges_exchange_07_classificationEx",
          "classHierarchy": "Quantities / Environmental quantities / EPD EN 15804 / LCI indicators",
          "nameClass": "GaBiCategories"
        }
      },
      {
        "id": "ILCDex:63a79af11ab0467745a808dc6fc9d4ca_exchanges_exchange_08",
        "dataSetInternalID": 7,
        "referenceToFlowDataSet": {
          "id": "ILCDex:63a79af11ab0467745a808dc6fc9d4ca_exchanges_exchange_08_referenceToFlowDataSet",
          "shortDescription": [
            {
              "id": "ILCDex:63a79af11ab0467745a808dc6fc9d4ca_exchanges_exchange_08_referenceToFlowDataSet_shortDescription_01",
              "value": "Use of secondary material (SM)",
              "lang": "en"
            }
          ],
          "type": "flow data set",
          "refObjectId": "c6a1f35f-2d09-4f54-8dfb-97e502e1ce92"
        },
        "meanAmount": 0.0,
        "resolvedFlowVersion": "35.00.000",
        "flowProperties": [],
        "typeOfFlow": "Other flow",
        "exchangeDirection": "INPUT",
        "otherEx": {
          "id": "ILCDex:63a79af11ab0467745a808dc6fc9d4ca_exchanges_exchange_08_otherEx",
          "anies": [
            {
              "id": "ILCDex:63a79af11ab0467745a808dc6fc9d4ca_exchanges_exchange_08_otherEx_anies_moduleA1",
              "value": "536.140987215737",
              "module": "A1"
            },
            {
              "id": "ILCDex:63a79af11ab0467745a808dc6fc9d4ca_exchanges_exchange_08_otherEx_anies_moduleA2",
              "value": "0",
              "module": "A2"
            },
            {
              "id": "ILCDex:63a79af11ab0467745a808dc6fc9d4ca_exchanges_exchange_08_otherEx_anies_moduleA3",
              "value": "0",
              "module": "A3"
            },
            {
              "id": "ILCDex:63a79af11ab0467745a808dc6fc9d4ca_exchanges_exchange_08_otherEx_anies_moduleA1A3",
              "value": "536.140987215737",
              "module": "A1-A3"
            },
            {
              "id": "ILCDex:63a79af11ab0467745a808dc6fc9d4ca_exchanges_exchange_08_otherEx_anies_moduleA4",
              "value": "ND",
              "module": "A4"
            },
            {
              "id": "ILCDex:63a79af11ab0467745a808dc6fc9d4ca_exchanges_exchange_08_otherEx_anies_moduleA5",
              "value": "ND",
              "module": "A5"
            },
            {
              "id": "ILCDex:63a79af11ab0467745a808dc6fc9d4ca_exchanges_exchange_08_otherEx_anies_moduleB1",
              "value": "0",
              "module": "B1"
            },
            {
              "id": "ILCDex:63a79af11ab0467745a808dc6fc9d4ca_exchanges_exchange_08_otherEx_anies_moduleB2",
              "value": "0",
              "module": "B2"
            },
            {
              "id": "ILCDex:63a79af11ab0467745a808dc6fc9d4ca_exchanges_exchange_08_otherEx_anies_moduleB3",
              "value": "0",
              "module": "B3"
            },
            {
              "id": "ILCDex:63a79af11ab0467745a808dc6fc9d4ca_exchanges_exchange_08_otherEx_anies_moduleB4",
              "value": "0",
              "module": "B4"
            },
            {
              "id": "ILCDex:63a79af11ab0467745a808dc6fc9d4ca_exchanges_exchange_08_otherEx_anies_moduleB5",
              "value": "0",
              "module": "B5"
            },
            {
              "id": "ILCDex:63a79af11ab0467745a808dc6fc9d4ca_exchanges_exchange_08_otherEx_anies_moduleB6",
              "value": "0",
              "module": "B6"
            },
            {
              "id": "ILCDex:63a79af11ab0467745a808dc6fc9d4ca_exchanges_exchange_08_otherEx_anies_moduleB7",
              "value": "0",
              "module": "B7"
            },
            {
              "id": "ILCDex:63a79af11ab0467745a808dc6fc9d4ca_exchanges_exchange_08_otherEx_anies_moduleC1",
              "value": "0",
              "module": "C1"
            },
            {
              "id": "ILCDex:63a79af11ab0467745a808dc6fc9d4ca_exchanges_exchange_08_otherEx_anies_moduleC2",
              "value": "0",
              "module": "C2"
            },
            {
              "id": "ILCDex:63a79af11ab0467745a808dc6fc9d4ca_exchanges_exchange_08_otherEx_anies_moduleC3",
              "value": "0",
              "module": "C3"
            },
            {
              "id": "ILCDex:63a79af11ab0467745a808dc6fc9d4ca_exchanges_exchange_08_otherEx_anies_moduleC4",
              "value": "0",
              "module": "C4"
            },
            {
              "id": "ILCDex:63a79af11ab0467745a808dc6fc9d4ca_exchanges_exchange_08_otherEx_anies_moduleD",
              "value": "0",
              "module": "D"
            },
            {
              "id": "ILCDex:63a79af11ab0467745a808dc6fc9d4ca_exchanges_exchange_08_otherEx_anies_19",
              "name": "referenceToUnitGroupDataSet",
              "objectValue": {
                "id": "ILCDex:63a79af11ab0467745a808dc6fc9d4ca_exchanges_exchange_08_otherEx_anies_19_objectValue",
                "shortDescription": [
                  {
                    "id": "ILCDex:63a79af11ab0467745a808dc6fc9d4ca_exchanges_exchange_08_otherEx_anies_19_objectValue_shortDescription_01",
                    "value": "kg"
                  }
                ],
                "type": "unit group data set",
                "refObjectId": "ad38d542-3fe9-439d-9b95-2f5f7752acaf",
                "refObjectUri": "../unitgroups/ad38d542-3fe9-439d-9b95-2f5f7752acaf"
              }
            }
          ]
        },
        "classificationEx": {
          "id": "ILCDex:63a79af11ab0467745a808dc6fc9d4ca_exchanges_exchange_08_classificationEx",
          "classHierarchy": "Quantities / Environmental quantities / EPD EN 15804 / LCI indicators",
          "nameClass": "GaBiCategories"
        }
      },
      {
        "id": "ILCDex:63a79af11ab0467745a808dc6fc9d4ca_exchanges_exchange_09",
        "dataSetInternalID": 8,
        "referenceToFlowDataSet": {
          "id": "ILCDex:63a79af11ab0467745a808dc6fc9d4ca_exchanges_exchange_09_referenceToFlowDataSet",
          "shortDescription": [
            {
              "id": "ILCDex:63a79af11ab0467745a808dc6fc9d4ca_exchanges_exchange_09_referenceToFlowDataSet_shortDescription_01",
              "value": "Use of renewable secondary fuels (RSF)",
              "lang": "en"
            }
          ],
          "type": "flow data set",
          "refObjectId": "64333088-a55f-4aa2-9a31-c10b07816787"
        },
        "meanAmount": 0.0,
        "resolvedFlowVersion": "30.00.000",
        "flowProperties": [],
        "typeOfFlow": "Other flow",
        "exchangeDirection": "INPUT",
        "otherEx": {
          "id": "ILCDex:63a79af11ab0467745a808dc6fc9d4ca_exchanges_exchange_09_otherEx",
          "anies": [
            {
              "id": "ILCDex:63a79af11ab0467745a808dc6fc9d4ca_exchanges_exchange_09_otherEx_anies_moduleA1",
              "value": "63.0392213775255",
              "module": "A1"
            },
            {
              "id": "ILCDex:63a79af11ab0467745a808dc6fc9d4ca_exchanges_exchange_09_otherEx_anies_moduleA2",
              "value": "0",
              "module": "A2"
            },
            {
              "id": "ILCDex:63a79af11ab0467745a808dc6fc9d4ca_exchanges_exchange_09_otherEx_anies_moduleA3",
              "value": "0",
              "module": "A3"
            },
            {
              "id": "ILCDex:63a79af11ab0467745a808dc6fc9d4ca_exchanges_exchange_09_otherEx_anies_moduleA1A3",
              "value": "63.0392213775255",
              "module": "A1-A3"
            },
            {
              "id": "ILCDex:63a79af11ab0467745a808dc6fc9d4ca_exchanges_exchange_09_otherEx_anies_moduleA4",
              "value": "ND",
              "module": "A4"
            },
            {
              "id": "ILCDex:63a79af11ab0467745a808dc6fc9d4ca_exchanges_exchange_09_otherEx_anies_moduleA5",
              "value": "ND",
              "module": "A5"
            },
            {
              "id": "ILCDex:63a79af11ab0467745a808dc6fc9d4ca_exchanges_exchange_09_otherEx_anies_moduleB1",
              "value": "0",
              "module": "B1"
            },
            {
              "id": "ILCDex:63a79af11ab0467745a808dc6fc9d4ca_exchanges_exchange_09_otherEx_anies_moduleB2",
              "value": "0",
              "module": "B2"
            },
            {
              "id": "ILCDex:63a79af11ab0467745a808dc6fc9d4ca_exchanges_exchange_09_otherEx_anies_moduleB3",
              "value": "0",
              "module": "B3"
            },
            {
              "id": "ILCDex:63a79af11ab0467745a808dc6fc9d4ca_exchanges_exchange_09_otherEx_anies_moduleB4",
              "value": "0",
              "module": "B4"
            },
            {
              "id": "ILCDex:63a79af11ab0467745a808dc6fc9d4ca_exchanges_exchange_09_otherEx_anies_moduleB5",
              "value": "0",
              "module": "B5"
            },
            {
              "id": "ILCDex:63a79af11ab0467745a808dc6fc9d4ca_exchanges_exchange_09_otherEx_anies_moduleB6",
              "value": "0",
              "module": "B6"
            },
            {
              "id": "ILCDex:63a79af11ab0467745a808dc6fc9d4ca_exchanges_exchange_09_otherEx_anies_moduleB7",
              "value": "0",
              "module": "B7"
            },
            {
              "id": "ILCDex:63a79af11ab0467745a808dc6fc9d4ca_exchanges_exchange_09_otherEx_anies_moduleC1",
              "value": "0",
              "module": "C1"
            },
            {
              "id": "ILCDex:63a79af11ab0467745a808dc6fc9d4ca_exchanges_exchange_09_otherEx_anies_moduleC2",
              "value": "0",
              "module": "C2"
            },
            {
              "id": "ILCDex:63a79af11ab0467745a808dc6fc9d4ca_exchanges_exchange_09_otherEx_anies_moduleC3",
              "value": "0",
              "module": "C3"
            },
            {
              "id": "ILCDex:63a79af11ab0467745a808dc6fc9d4ca_exchanges_exchange_09_otherEx_anies_moduleC4",
              "value": "0",
              "module": "C4"
            },
            {
              "id": "ILCDex:63a79af11ab0467745a808dc6fc9d4ca_exchanges_exchange_09_otherEx_anies_moduleD",
              "value": "0",
              "module": "D"
            },
            {
              "id": "ILCDex:63a79af11ab0467745a808dc6fc9d4ca_exchanges_exchange_09_otherEx_anies_19",
              "name": "referenceToUnitGroupDataSet",
              "objectValue": {
                "id": "ILCDex:63a79af11ab0467745a808dc6fc9d4ca_exchanges_exchange_09_otherEx_anies_19_objectValue",
                "shortDescription": [
                  {
                    "id": "ILCDex:63a79af11ab0467745a808dc6fc9d4ca_exchanges_exchange_09_otherEx_anies_19_objectValue_shortDescription_01",
                    "value": "MJ"
                  }
                ],
                "type": "unit group data set",
                "refObjectId": "93a60a57-a3c8-11da-a746-0800200c9a66",
                "refObjectUri": "../unitgroups/93a60a57-a3c8-11da-a746-0800200c9a66"
              }
            }
          ]
        },
        "classificationEx": {
          "id": "ILCDex:63a79af11ab0467745a808dc6fc9d4ca_exchanges_exchange_09_classificationEx",
          "classHierarchy": "Größen / Umweltliche Größen / EPD EN 15804 / LCI Indikatoren",
          "nameClass": "GaBiCategories"
        }
      },
      {
        "id": "ILCDex:63a79af11ab0467745a808dc6fc9d4ca_exchanges_exchange_10",
        "dataSetInternalID": 9,
        "referenceToFlowDataSet": {
          "id": "ILCDex:63a79af11ab0467745a808dc6fc9d4ca_exchanges_exchange_10_referenceToFlowDataSet",
          "shortDescription": [
            {
              "id": "ILCDex:63a79af11ab0467745a808dc6fc9d4ca_exchanges_exchange_10_referenceToFlowDataSet_shortDescription_01",
              "value": "Use of non renewable secondary fuels (NRSF)",
              "lang": "en"
            }
          ],
          "type": "flow data set",
          "refObjectId": "89def144-d39a-4287-b86f-efde453ddcb2"
        },
        "meanAmount": 0.0,
        "resolvedFlowVersion": "30.00.000",
        "flowProperties": [],
        "typeOfFlow": "Other flow",
        "exchangeDirection": "INPUT",
        "otherEx": {
          "id": "ILCDex:63a79af11ab0467745a808dc6fc9d4ca_exchanges_exchange_10_otherEx",
          "anies": [
            {
              "id": "ILCDex:63a79af11ab0467745a808dc6fc9d4ca_exchanges_exchange_10_otherEx_anies_moduleA1",
              "value": "87.9090848380632",
              "module": "A1"
            },
            {
              "id": "ILCDex:63a79af11ab0467745a808dc6fc9d4ca_exchanges_exchange_10_otherEx_anies_moduleA2",
              "value": "0",
              "module": "A2"
            },
            {
              "id": "ILCDex:63a79af11ab0467745a808dc6fc9d4ca_exchanges_exchange_10_otherEx_anies_moduleA3",
              "value": "0",
              "module": "A3"
            },
            {
              "id": "ILCDex:63a79af11ab0467745a808dc6fc9d4ca_exchanges_exchange_10_otherEx_anies_moduleA1A3",
              "value": "87.9090848380632",
              "module": "A1-A3"
            },
            {
              "id": "ILCDex:63a79af11ab0467745a808dc6fc9d4ca_exchanges_exchange_10_otherEx_anies_moduleA4",
              "value": "ND",
              "module": "A4"
            },
            {
              "id": "ILCDex:63a79af11ab0467745a808dc6fc9d4ca_exchanges_exchange_10_otherEx_anies_moduleA5",
              "value": "ND",
              "module": "A5"
            },
            {
              "id": "ILCDex:63a79af11ab0467745a808dc6fc9d4ca_exchanges_exchange_10_otherEx_anies_moduleB1",
              "value": "0",
              "module": "B1"
            },
            {
              "id": "ILCDex:63a79af11ab0467745a808dc6fc9d4ca_exchanges_exchange_10_otherEx_anies_moduleB2",
              "value": "0",
              "module": "B2"
            },
            {
              "id": "ILCDex:63a79af11ab0467745a808dc6fc9d4ca_exchanges_exchange_10_otherEx_anies_moduleB3",
              "value": "0",
              "module": "B3"
            },
            {
              "id": "ILCDex:63a79af11ab0467745a808dc6fc9d4ca_exchanges_exchange_10_otherEx_anies_moduleB4",
              "value": "0",
              "module": "B4"
            },
            {
              "id": "ILCDex:63a79af11ab0467745a808dc6fc9d4ca_exchanges_exchange_10_otherEx_anies_moduleB5",
              "value": "0",
              "module": "B5"
            },
            {
              "id": "ILCDex:63a79af11ab0467745a808dc6fc9d4ca_exchanges_exchange_10_otherEx_anies_moduleB6",
              "value": "0",
              "module": "B6"
            },
            {
              "id": "ILCDex:63a79af11ab0467745a808dc6fc9d4ca_exchanges_exchange_10_otherEx_anies_moduleB7",
              "value": "0",
              "module": "B7"
            },
            {
              "id": "ILCDex:63a79af11ab0467745a808dc6fc9d4ca_exchanges_exchange_10_otherEx_anies_moduleC1",
              "value": "0",
              "module": "C1"
            },
            {
              "id": "ILCDex:63a79af11ab0467745a808dc6fc9d4ca_exchanges_exchange_10_otherEx_anies_moduleC2",
              "value": "0",
              "module": "C2"
            },
            {
              "id": "ILCDex:63a79af11ab0467745a808dc6fc9d4ca_exchanges_exchange_10_otherEx_anies_moduleC3",
              "value": "0",
              "module": "C3"
            },
            {
              "id": "ILCDex:63a79af11ab0467745a808dc6fc9d4ca_exchanges_exchange_10_otherEx_anies_moduleC4",
              "value": "0",
              "module": "C4"
            },
            {
              "id": "ILCDex:63a79af11ab0467745a808dc6fc9d4ca_exchanges_exchange_10_otherEx_anies_moduleD",
              "value": "0",
              "module": "D"
            },
            {
              "id": "ILCDex:63a79af11ab0467745a808dc6fc9d4ca_exchanges_exchange_10_otherEx_anies_19",
              "name": "referenceToUnitGroupDataSet",
              "objectValue": {
                "id": "ILCDex:63a79af11ab0467745a808dc6fc9d4ca_exchanges_exchange_10_otherEx_anies_19_objectValue",
                "shortDescription": [
                  {
                    "id": "ILCDex:63a79af11ab0467745a808dc6fc9d4ca_exchanges_exchange_10_otherEx_anies_19_objectValue_shortDescription_01",
                    "value": "MJ"
                  }
                ],
                "type": "unit group data set",
                "refObjectId": "93a60a57-a3c8-11da-a746-0800200c9a66",
                "refObjectUri": "../unitgroups/93a60a57-a3c8-11da-a746-0800200c9a66"
              }
            }
          ]
        },
        "classificationEx": {
          "id": "ILCDex:63a79af11ab0467745a808dc6fc9d4ca_exchanges_exchange_10_classificationEx",
          "classHierarchy": "Größen / Umweltliche Größen / EPD EN 15804 / LCI Indikatoren",
          "nameClass": "GaBiCategories"
        }
      },
      {
        "id": "ILCDex:63a79af11ab0467745a808dc6fc9d4ca_exchanges_exchange_11",
        "dataSetInternalID": 10,
        "referenceToFlowDataSet": {
          "id": "ILCDex:63a79af11ab0467745a808dc6fc9d4ca_exchanges_exchange_11_referenceToFlowDataSet",
          "shortDescription": [
            {
              "id": "ILCDex:63a79af11ab0467745a808dc6fc9d4ca_exchanges_exchange_11_referenceToFlowDataSet_shortDescription_01",
              "value": "Net use of fresh water (FW)",
              "lang": "en"
            }
          ],
          "type": "flow data set",
          "refObjectId": "3cf952c8-f3a4-461d-8c96-96456ca62246"
        },
        "meanAmount": 0.0,
        "resolvedFlowVersion": "35.00.000",
        "flowProperties": [],
        "typeOfFlow": "Other flow",
        "exchangeDirection": "INPUT",
        "otherEx": {
          "id": "ILCDex:63a79af11ab0467745a808dc6fc9d4ca_exchanges_exchange_11_otherEx",
          "anies": [
            {
              "id": "ILCDex:63a79af11ab0467745a808dc6fc9d4ca_exchanges_exchange_11_otherEx_anies_moduleA1",
              "value": "1.83530005474822",
              "module": "A1"
            },
            {
              "id": "ILCDex:63a79af11ab0467745a808dc6fc9d4ca_exchanges_exchange_11_otherEx_anies_moduleA2",
              "value": "0.0381419579383361",
              "module": "A2"
            },
            {
              "id": "ILCDex:63a79af11ab0467745a808dc6fc9d4ca_exchanges_exchange_11_otherEx_anies_moduleA3",
              "value": "0.0601138975028198",
              "module": "A3"
            },
            {
              "id": "ILCDex:63a79af11ab0467745a808dc6fc9d4ca_exchanges_exchange_11_otherEx_anies_moduleA1A3",
              "value": "1.93355591018938",
              "module": "A1-A3"
            },
            {
              "id": "ILCDex:63a79af11ab0467745a808dc6fc9d4ca_exchanges_exchange_11_otherEx_anies_moduleA4",
              "value": "ND",
              "module": "A4"
            },
            {
              "id": "ILCDex:63a79af11ab0467745a808dc6fc9d4ca_exchanges_exchange_11_otherEx_anies_moduleA5",
              "value": "ND",
              "module": "A5"
            },
            {
              "id": "ILCDex:63a79af11ab0467745a808dc6fc9d4ca_exchanges_exchange_11_otherEx_anies_moduleB1",
              "value": "0",
              "module": "B1"
            },
            {
              "id": "ILCDex:63a79af11ab0467745a808dc6fc9d4ca_exchanges_exchange_11_otherEx_anies_moduleB2",
              "value": "0",
              "module": "B2"
            },
            {
              "id": "ILCDex:63a79af11ab0467745a808dc6fc9d4ca_exchanges_exchange_11_otherEx_anies_moduleB3",
              "value": "0",
              "module": "B3"
            },
            {
              "id": "ILCDex:63a79af11ab0467745a808dc6fc9d4ca_exchanges_exchange_11_otherEx_anies_moduleB4",
              "value": "0",
              "module": "B4"
            },
            {
              "id": "ILCDex:63a79af11ab0467745a808dc6fc9d4ca_exchanges_exchange_11_otherEx_anies_moduleB5",
              "value": "0",
              "module": "B5"
            },
            {
              "id": "ILCDex:63a79af11ab0467745a808dc6fc9d4ca_exchanges_exchange_11_otherEx_anies_moduleB6",
              "value": "0",
              "module": "B6"
            },
            {
              "id": "ILCDex:63a79af11ab0467745a808dc6fc9d4ca_exchanges_exchange_11_otherEx_anies_moduleB7",
              "value": "0",
              "module": "B7"
            },
            {
              "id": "ILCDex:63a79af11ab0467745a808dc6fc9d4ca_exchanges_exchange_11_otherEx_anies_moduleC1",
              "value": "0.019933565638",
              "module": "C1"
            },
            {
              "id": "ILCDex:63a79af11ab0467745a808dc6fc9d4ca_exchanges_exchange_11_otherEx_anies_moduleC2",
              "value": "0.037784055375",
              "module": "C2"
            },
            {
              "id": "ILCDex:63a79af11ab0467745a808dc6fc9d4ca_exchanges_exchange_11_otherEx_anies_moduleC3",
              "value": "0.04678641",
              "module": "C3"
            },
            {
              "id": "ILCDex:63a79af11ab0467745a808dc6fc9d4ca_exchanges_exchange_11_otherEx_anies_moduleC4",
              "value": "0.084679330725",
              "module": "C4"
            },
            {
              "id": "ILCDex:63a79af11ab0467745a808dc6fc9d4ca_exchanges_exchange_11_otherEx_anies_moduleD",
              "value": "-0.703542710475",
              "module": "D"
            },
            {
              "id": "ILCDex:63a79af11ab0467745a808dc6fc9d4ca_exchanges_exchange_11_otherEx_anies_19",
              "name": "referenceToUnitGroupDataSet",
              "objectValue": {
                "id": "ILCDex:63a79af11ab0467745a808dc6fc9d4ca_exchanges_exchange_11_otherEx_anies_19_objectValue",
                "shortDescription": [
                  {
                    "id": "ILCDex:63a79af11ab0467745a808dc6fc9d4ca_exchanges_exchange_11_otherEx_anies_19_objectValue_shortDescription_01",
                    "value": "m3"
                  }
                ],
                "type": "unit group data set",
                "refObjectId": "cd950537-0a98-4044-9ba7-9f9a68d0a504",
                "refObjectUri": "../unitgroups/cd950537-0a98-4044-9ba7-9f9a68d0a504"
              }
            }
          ]
        },
        "classificationEx": {
          "id": "ILCDex:63a79af11ab0467745a808dc6fc9d4ca_exchanges_exchange_11_classificationEx",
          "classHierarchy": "Quantities / Environmental quantities / EPD EN 15804 / LCI indicators",
          "nameClass": "GaBiCategories"
        }
      },
      {
        "id": "ILCDex:63a79af11ab0467745a808dc6fc9d4ca_exchanges_exchange_12",
        "dataSetInternalID": 11,
        "referenceToFlowDataSet": {
          "id": "ILCDex:63a79af11ab0467745a808dc6fc9d4ca_exchanges_exchange_12_referenceToFlowDataSet",
          "shortDescription": [
            {
              "id": "ILCDex:63a79af11ab0467745a808dc6fc9d4ca_exchanges_exchange_12_referenceToFlowDataSet_shortDescription_01",
              "value": "Hazardous waste disposed (HWD)",
              "lang": "en"
            }
          ],
          "type": "flow data set",
          "refObjectId": "430f9e0f-59b2-46a0-8e0d-55e0e84948fc"
        },
        "meanAmount": 0.0,
        "resolvedFlowVersion": "35.00.000",
        "flowProperties": [],
        "typeOfFlow": "Other flow",
        "exchangeDirection": "OUTPUT",
        "otherEx": {
          "id": "ILCDex:63a79af11ab0467745a808dc6fc9d4ca_exchanges_exchange_12_otherEx",
          "anies": [
            {
              "id": "ILCDex:63a79af11ab0467745a808dc6fc9d4ca_exchanges_exchange_12_otherEx_anies_moduleA1",
              "value": "0.0324168484932",
              "module": "A1"
            },
            {
              "id": "ILCDex:63a79af11ab0467745a808dc6fc9d4ca_exchanges_exchange_12_otherEx_anies_moduleA2",
              "value": "0",
              "module": "A2"
            },
            {
              "id": "ILCDex:63a79af11ab0467745a808dc6fc9d4ca_exchanges_exchange_12_otherEx_anies_moduleA3",
              "value": "0",
              "module": "A3"
            },
            {
              "id": "ILCDex:63a79af11ab0467745a808dc6fc9d4ca_exchanges_exchange_12_otherEx_anies_moduleA1A3",
              "value": "0.0324168484932",
              "module": "A1-A3"
            },
            {
              "id": "ILCDex:63a79af11ab0467745a808dc6fc9d4ca_exchanges_exchange_12_otherEx_anies_moduleA4",
              "value": "ND",
              "module": "A4"
            },
            {
              "id": "ILCDex:63a79af11ab0467745a808dc6fc9d4ca_exchanges_exchange_12_otherEx_anies_moduleA5",
              "value": "ND",
              "module": "A5"
            },
            {
              "id": "ILCDex:63a79af11ab0467745a808dc6fc9d4ca_exchanges_exchange_12_otherEx_anies_moduleB1",
              "value": "0",
              "module": "B1"
            },
            {
              "id": "ILCDex:63a79af11ab0467745a808dc6fc9d4ca_exchanges_exchange_12_otherEx_anies_moduleB2",
              "value": "0",
              "module": "B2"
            },
            {
              "id": "ILCDex:63a79af11ab0467745a808dc6fc9d4ca_exchanges_exchange_12_otherEx_anies_moduleB3",
              "value": "0",
              "module": "B3"
            },
            {
              "id": "ILCDex:63a79af11ab0467745a808dc6fc9d4ca_exchanges_exchange_12_otherEx_anies_moduleB4",
              "value": "0",
              "module": "B4"
            },
            {
              "id": "ILCDex:63a79af11ab0467745a808dc6fc9d4ca_exchanges_exchange_12_otherEx_anies_moduleB5",
              "value": "0",
              "module": "B5"
            },
            {
              "id": "ILCDex:63a79af11ab0467745a808dc6fc9d4ca_exchanges_exchange_12_otherEx_anies_moduleB6",
              "value": "0",
              "module": "B6"
            },
            {
              "id": "ILCDex:63a79af11ab0467745a808dc6fc9d4ca_exchanges_exchange_12_otherEx_anies_moduleB7",
              "value": "0",
              "module": "B7"
            },
            {
              "id": "ILCDex:63a79af11ab0467745a808dc6fc9d4ca_exchanges_exchange_12_otherEx_anies_moduleC1",
              "value": "0",
              "module": "C1"
            },
            {
              "id": "ILCDex:63a79af11ab0467745a808dc6fc9d4ca_exchanges_exchange_12_otherEx_anies_moduleC2",
              "value": "0",
              "module": "C2"
            },
            {
              "id": "ILCDex:63a79af11ab0467745a808dc6fc9d4ca_exchanges_exchange_12_otherEx_anies_moduleC3",
              "value": "0",
              "module": "C3"
            },
            {
              "id": "ILCDex:63a79af11ab0467745a808dc6fc9d4ca_exchanges_exchange_12_otherEx_anies_moduleC4",
              "value": "0",
              "module": "C4"
            },
            {
              "id": "ILCDex:63a79af11ab0467745a808dc6fc9d4ca_exchanges_exchange_12_otherEx_anies_moduleD",
              "value": "0",
              "module": "D"
            },
            {
              "id": "ILCDex:63a79af11ab0467745a808dc6fc9d4ca_exchanges_exchange_12_otherEx_anies_19",
              "name": "referenceToUnitGroupDataSet",
              "objectValue": {
                "id": "ILCDex:63a79af11ab0467745a808dc6fc9d4ca_exchanges_exchange_12_otherEx_anies_19_objectValue",
                "shortDescription": [
                  {
                    "id": "ILCDex:63a79af11ab0467745a808dc6fc9d4ca_exchanges_exchange_12_otherEx_anies_19_objectValue_shortDescription_01",
                    "value": "kg"
                  }
                ],
                "type": "unit group data set",
                "refObjectId": "ad38d542-3fe9-439d-9b95-2f5f7752acaf",
                "refObjectUri": "../unitgroups/ad38d542-3fe9-439d-9b95-2f5f7752acaf"
              }
            }
          ]
        },
        "classificationEx": {
          "id": "ILCDex:63a79af11ab0467745a808dc6fc9d4ca_exchanges_exchange_12_classificationEx",
          "classHierarchy": "Quantities / Environmental quantities / EPD EN 15804 / LCI indicators",
          "nameClass": "GaBiCategories"
        }
      },
      {
        "id": "ILCDex:63a79af11ab0467745a808dc6fc9d4ca_exchanges_exchange_13",
        "dataSetInternalID": 12,
        "referenceToFlowDataSet": {
          "id": "ILCDex:63a79af11ab0467745a808dc6fc9d4ca_exchanges_exchange_13_referenceToFlowDataSet",
          "shortDescription": [
            {
              "id": "ILCDex:63a79af11ab0467745a808dc6fc9d4ca_exchanges_exchange_13_referenceToFlowDataSet_shortDescription_01",
              "value": "Non harzardous waste disposed (NHWD)",
              "lang": "en"
            }
          ],
          "type": "flow data set",
          "refObjectId": "b29ef66b-e286-4afa-949f-62f1a7b4d7fa"
        },
        "meanAmount": 0.0,
        "resolvedFlowVersion": "35.00.000",
        "flowProperties": [],
        "typeOfFlow": "Other flow",
        "exchangeDirection": "OUTPUT",
        "otherEx": {
          "id": "ILCDex:63a79af11ab0467745a808dc6fc9d4ca_exchanges_exchange_13_otherEx",
          "anies": [
            {
              "id": "ILCDex:63a79af11ab0467745a808dc6fc9d4ca_exchanges_exchange_13_otherEx_anies_moduleA1",
              "value": "0.0004178068349",
              "module": "A1"
            },
            {
              "id": "ILCDex:63a79af11ab0467745a808dc6fc9d4ca_exchanges_exchange_13_otherEx_anies_moduleA2",
              "value": "0",
              "module": "A2"
            },
            {
              "id": "ILCDex:63a79af11ab0467745a808dc6fc9d4ca_exchanges_exchange_13_otherEx_anies_moduleA3",
              "value": "0.12",
              "module": "A3"
            },
            {
              "id": "ILCDex:63a79af11ab0467745a808dc6fc9d4ca_exchanges_exchange_13_otherEx_anies_moduleA1A3",
              "value": "0.1204178068349",
              "module": "A1-A3"
            },
            {
              "id": "ILCDex:63a79af11ab0467745a808dc6fc9d4ca_exchanges_exchange_13_otherEx_anies_moduleA4",
              "value": "ND",
              "module": "A4"
            },
            {
              "id": "ILCDex:63a79af11ab0467745a808dc6fc9d4ca_exchanges_exchange_13_otherEx_anies_moduleA5",
              "value": "ND",
              "module": "A5"
            },
            {
              "id": "ILCDex:63a79af11ab0467745a808dc6fc9d4ca_exchanges_exchange_13_otherEx_anies_moduleB1",
              "value": "0",
              "module": "B1"
            },
            {
              "id": "ILCDex:63a79af11ab0467745a808dc6fc9d4ca_exchanges_exchange_13_otherEx_anies_moduleB2",
              "value": "0",
              "module": "B2"
            },
            {
              "id": "ILCDex:63a79af11ab0467745a808dc6fc9d4ca_exchanges_exchange_13_otherEx_anies_moduleB3",
              "value": "0",
              "module": "B3"
            },
            {
              "id": "ILCDex:63a79af11ab0467745a808dc6fc9d4ca_exchanges_exchange_13_otherEx_anies_moduleB4",
              "value": "0",
              "module": "B4"
            },
            {
              "id": "ILCDex:63a79af11ab0467745a808dc6fc9d4ca_exchanges_exchange_13_otherEx_anies_moduleB5",
              "value": "0",
              "module": "B5"
            },
            {
              "id": "ILCDex:63a79af11ab0467745a808dc6fc9d4ca_exchanges_exchange_13_otherEx_anies_moduleB6",
              "value": "0",
              "module": "B6"
            },
            {
              "id": "ILCDex:63a79af11ab0467745a808dc6fc9d4ca_exchanges_exchange_13_otherEx_anies_moduleB7",
              "value": "0",
              "module": "B7"
            },
            {
              "id": "ILCDex:63a79af11ab0467745a808dc6fc9d4ca_exchanges_exchange_13_otherEx_anies_moduleC1",
              "value": "0",
              "module": "C1"
            },
            {
              "id": "ILCDex:63a79af11ab0467745a808dc6fc9d4ca_exchanges_exchange_13_otherEx_anies_moduleC2",
              "value": "0",
              "module": "C2"
            },
            {
              "id": "ILCDex:63a79af11ab0467745a808dc6fc9d4ca_exchanges_exchange_13_otherEx_anies_moduleC3",
              "value": "0",
              "module": "C3"
            },
            {
              "id": "ILCDex:63a79af11ab0467745a808dc6fc9d4ca_exchanges_exchange_13_otherEx_anies_moduleC4",
              "value": "486.525",
              "module": "C4"
            },
            {
              "id": "ILCDex:63a79af11ab0467745a808dc6fc9d4ca_exchanges_exchange_13_otherEx_anies_moduleD",
              "value": "0",
              "module": "D"
            },
            {
              "id": "ILCDex:63a79af11ab0467745a808dc6fc9d4ca_exchanges_exchange_13_otherEx_anies_19",
              "name": "referenceToUnitGroupDataSet",
              "objectValue": {
                "id": "ILCDex:63a79af11ab0467745a808dc6fc9d4ca_exchanges_exchange_13_otherEx_anies_19_objectValue",
                "shortDescription": [
                  {
                    "id": "ILCDex:63a79af11ab0467745a808dc6fc9d4ca_exchanges_exchange_13_otherEx_anies_19_objectValue_shortDescription_01",
                    "value": "kg"
                  }
                ],
                "type": "unit group data set",
                "refObjectId": "ad38d542-3fe9-439d-9b95-2f5f7752acaf",
                "refObjectUri": "../unitgroups/ad38d542-3fe9-439d-9b95-2f5f7752acaf"
              }
            }
          ]
        },
        "classificationEx": {
          "id": "ILCDex:63a79af11ab0467745a808dc6fc9d4ca_exchanges_exchange_13_classificationEx",
          "classHierarchy": "Quantities / Environmental quantities / EPD EN 15804 / LCI indicators",
          "nameClass": "GaBiCategories"
        }
      },
      {
        "id": "ILCDex:63a79af11ab0467745a808dc6fc9d4ca_exchanges_exchange_14",
        "dataSetInternalID": 13,
        "referenceToFlowDataSet": {
          "id": "ILCDex:63a79af11ab0467745a808dc6fc9d4ca_exchanges_exchange_14_referenceToFlowDataSet",
          "shortDescription": [
            {
              "id": "ILCDex:63a79af11ab0467745a808dc6fc9d4ca_exchanges_exchange_14_referenceToFlowDataSet_shortDescription_01",
              "value": "Radioactive waste disposed (RWD)",
              "lang": "en"
            }
          ],
          "type": "flow data set",
          "refObjectId": "3449546e-52ad-4b39-b809-9fb77cea8ff6"
        },
        "meanAmount": 0.0,
        "resolvedFlowVersion": "35.00.000",
        "flowProperties": [],
        "typeOfFlow": "Other flow",
        "exchangeDirection": "OUTPUT",
        "otherEx": {
          "id": "ILCDex:63a79af11ab0467745a808dc6fc9d4ca_exchanges_exchange_14_otherEx",
          "anies": [
            {
              "id": "ILCDex:63a79af11ab0467745a808dc6fc9d4ca_exchanges_exchange_14_otherEx_anies_moduleA1",
              "value": "0",
              "module": "A1"
            },
            {
              "id": "ILCDex:63a79af11ab0467745a808dc6fc9d4ca_exchanges_exchange_14_otherEx_anies_moduleA2",
              "value": "0",
              "module": "A2"
            },
            {
              "id": "ILCDex:63a79af11ab0467745a808dc6fc9d4ca_exchanges_exchange_14_otherEx_anies_moduleA3",
              "value": "0",
              "module": "A3"
            },
            {
              "id": "ILCDex:63a79af11ab0467745a808dc6fc9d4ca_exchanges_exchange_14_otherEx_anies_moduleA1A3",
              "value": "0",
              "module": "A1-A3"
            },
            {
              "id": "ILCDex:63a79af11ab0467745a808dc6fc9d4ca_exchanges_exchange_14_otherEx_anies_moduleA4",
              "value": "ND",
              "module": "A4"
            },
            {
              "id": "ILCDex:63a79af11ab0467745a808dc6fc9d4ca_exchanges_exchange_14_otherEx_anies_moduleA5",
              "value": "ND",
              "module": "A5"
            },
            {
              "id": "ILCDex:63a79af11ab0467745a808dc6fc9d4ca_exchanges_exchange_14_otherEx_anies_moduleB1",
              "value": "0",
              "module": "B1"
            },
            {
              "id": "ILCDex:63a79af11ab0467745a808dc6fc9d4ca_exchanges_exchange_14_otherEx_anies_moduleB2",
              "value": "0",
              "module": "B2"
            },
            {
              "id": "ILCDex:63a79af11ab0467745a808dc6fc9d4ca_exchanges_exchange_14_otherEx_anies_moduleB3",
              "value": "0",
              "module": "B3"
            },
            {
              "id": "ILCDex:63a79af11ab0467745a808dc6fc9d4ca_exchanges_exchange_14_otherEx_anies_moduleB4",
              "value": "0",
              "module": "B4"
            },
            {
              "id": "ILCDex:63a79af11ab0467745a808dc6fc9d4ca_exchanges_exchange_14_otherEx_anies_moduleB5",
              "value": "0",
              "module": "B5"
            },
            {
              "id": "ILCDex:63a79af11ab0467745a808dc6fc9d4ca_exchanges_exchange_14_otherEx_anies_moduleB6",
              "value": "0",
              "module": "B6"
            },
            {
              "id": "ILCDex:63a79af11ab0467745a808dc6fc9d4ca_exchanges_exchange_14_otherEx_anies_moduleB7",
              "value": "0",
              "module": "B7"
            },
            {
              "id": "ILCDex:63a79af11ab0467745a808dc6fc9d4ca_exchanges_exchange_14_otherEx_anies_moduleC1",
              "value": "0",
              "module": "C1"
            },
            {
              "id": "ILCDex:63a79af11ab0467745a808dc6fc9d4ca_exchanges_exchange_14_otherEx_anies_moduleC2",
              "value": "0",
              "module": "C2"
            },
            {
              "id": "ILCDex:63a79af11ab0467745a808dc6fc9d4ca_exchanges_exchange_14_otherEx_anies_moduleC3",
              "value": "0",
              "module": "C3"
            },
            {
              "id": "ILCDex:63a79af11ab0467745a808dc6fc9d4ca_exchanges_exchange_14_otherEx_anies_moduleC4",
              "value": "0",
              "module": "C4"
            },
            {
              "id": "ILCDex:63a79af11ab0467745a808dc6fc9d4ca_exchanges_exchange_14_otherEx_anies_moduleD",
              "value": "0",
              "module": "D"
            },
            {
              "id": "ILCDex:63a79af11ab0467745a808dc6fc9d4ca_exchanges_exchange_14_otherEx_anies_19",
              "name": "referenceToUnitGroupDataSet",
              "objectValue": {
                "id": "ILCDex:63a79af11ab0467745a808dc6fc9d4ca_exchanges_exchange_14_otherEx_anies_19_objectValue",
                "shortDescription": [
                  {
                    "id": "ILCDex:63a79af11ab0467745a808dc6fc9d4ca_exchanges_exchange_14_otherEx_anies_19_objectValue_shortDescription_01",
                    "value": "kg"
                  }
                ],
                "type": "unit group data set",
                "refObjectId": "ad38d542-3fe9-439d-9b95-2f5f7752acaf",
                "refObjectUri": "../unitgroups/ad38d542-3fe9-439d-9b95-2f5f7752acaf"
              }
            }
          ]
        },
        "classificationEx": {
          "id": "ILCDex:63a79af11ab0467745a808dc6fc9d4ca_exchanges_exchange_14_classificationEx",
          "classHierarchy": "Quantities / Environmental quantities / EPD EN 15804 / LCI indicators",
          "nameClass": "GaBiCategories"
        }
      },
      {
        "id": "ILCDex:63a79af11ab0467745a808dc6fc9d4ca_exchanges_exchange_15",
        "dataSetInternalID": 14,
        "referenceToFlowDataSet": {
          "id": "ILCDex:63a79af11ab0467745a808dc6fc9d4ca_exchanges_exchange_15_referenceToFlowDataSet",
          "shortDescription": [
            {
              "id": "ILCDex:63a79af11ab0467745a808dc6fc9d4ca_exchanges_exchange_15_referenceToFlowDataSet_shortDescription_01",
              "value": "Components for re-use (CRU)",
              "lang": "en"
            }
          ],
          "type": "flow data set",
          "refObjectId": "a2b32f97-3fc7-4af2-b209-525bc6426f33"
        },
        "meanAmount": 0.0,
        "resolvedFlowVersion": "30.00.000",
        "flowProperties": [],
        "typeOfFlow": "Other flow",
        "exchangeDirection": "OUTPUT",
        "otherEx": {
          "id": "ILCDex:63a79af11ab0467745a808dc6fc9d4ca_exchanges_exchange_15_otherEx",
          "anies": [
            {
              "id": "ILCDex:63a79af11ab0467745a808dc6fc9d4ca_exchanges_exchange_15_otherEx_anies_moduleA1",
              "value": "0",
              "module": "A1"
            },
            {
              "id": "ILCDex:63a79af11ab0467745a808dc6fc9d4ca_exchanges_exchange_15_otherEx_anies_moduleA2",
              "value": "0",
              "module": "A2"
            },
            {
              "id": "ILCDex:63a79af11ab0467745a808dc6fc9d4ca_exchanges_exchange_15_otherEx_anies_moduleA3",
              "value": "0",
              "module": "A3"
            },
            {
              "id": "ILCDex:63a79af11ab0467745a808dc6fc9d4ca_exchanges_exchange_15_otherEx_anies_moduleA1A3",
              "value": "0",
              "module": "A1-A3"
            },
            {
              "id": "ILCDex:63a79af11ab0467745a808dc6fc9d4ca_exchanges_exchange_15_otherEx_anies_moduleA4",
              "value": "ND",
              "module": "A4"
            },
            {
              "id": "ILCDex:63a79af11ab0467745a808dc6fc9d4ca_exchanges_exchange_15_otherEx_anies_moduleA5",
              "value": "ND",
              "module": "A5"
            },
            {
              "id": "ILCDex:63a79af11ab0467745a808dc6fc9d4ca_exchanges_exchange_15_otherEx_anies_moduleB1",
              "value": "0",
              "module": "B1"
            },
            {
              "id": "ILCDex:63a79af11ab0467745a808dc6fc9d4ca_exchanges_exchange_15_otherEx_anies_moduleB2",
              "value": "0",
              "module": "B2"
            },
            {
              "id": "ILCDex:63a79af11ab0467745a808dc6fc9d4ca_exchanges_exchange_15_otherEx_anies_moduleB3",
              "value": "0",
              "module": "B3"
            },
            {
              "id": "ILCDex:63a79af11ab0467745a808dc6fc9d4ca_exchanges_exchange_15_otherEx_anies_moduleB4",
              "value": "0",
              "module": "B4"
            },
            {
              "id": "ILCDex:63a79af11ab0467745a808dc6fc9d4ca_exchanges_exchange_15_otherEx_anies_moduleB5",
              "value": "0",
              "module": "B5"
            },
            {
              "id": "ILCDex:63a79af11ab0467745a808dc6fc9d4ca_exchanges_exchange_15_otherEx_anies_moduleB6",
              "value": "0",
              "module": "B6"
            },
            {
              "id": "ILCDex:63a79af11ab0467745a808dc6fc9d4ca_exchanges_exchange_15_otherEx_anies_moduleB7",
              "value": "0",
              "module": "B7"
            },
            {
              "id": "ILCDex:63a79af11ab0467745a808dc6fc9d4ca_exchanges_exchange_15_otherEx_anies_moduleC1",
              "value": "0",
              "module": "C1"
            },
            {
              "id": "ILCDex:63a79af11ab0467745a808dc6fc9d4ca_exchanges_exchange_15_otherEx_anies_moduleC2",
              "value": "0",
              "module": "C2"
            },
            {
              "id": "ILCDex:63a79af11ab0467745a808dc6fc9d4ca_exchanges_exchange_15_otherEx_anies_moduleC3",
              "value": "0",
              "module": "C3"
            },
            {
              "id": "ILCDex:63a79af11ab0467745a808dc6fc9d4ca_exchanges_exchange_15_otherEx_anies_moduleC4",
              "value": "0",
              "module": "C4"
            },
            {
              "id": "ILCDex:63a79af11ab0467745a808dc6fc9d4ca_exchanges_exchange_15_otherEx_anies_moduleD",
              "value": "0",
              "module": "D"
            },
            {
              "id": "ILCDex:63a79af11ab0467745a808dc6fc9d4ca_exchanges_exchange_15_otherEx_anies_19",
              "name": "referenceToUnitGroupDataSet",
              "objectValue": {
                "id": "ILCDex:63a79af11ab0467745a808dc6fc9d4ca_exchanges_exchange_15_otherEx_anies_19_objectValue",
                "shortDescription": [
                  {
                    "id": "ILCDex:63a79af11ab0467745a808dc6fc9d4ca_exchanges_exchange_15_otherEx_anies_19_objectValue_shortDescription_01",
                    "value": "kg"
                  }
                ],
                "type": "unit group data set",
                "refObjectId": "ad38d542-3fe9-439d-9b95-2f5f7752acaf",
                "refObjectUri": "../unitgroups/ad38d542-3fe9-439d-9b95-2f5f7752acaf"
              }
            }
          ]
        },
        "classificationEx": {
          "id": "ILCDex:63a79af11ab0467745a808dc6fc9d4ca_exchanges_exchange_15_classificationEx",
          "classHierarchy": "Größen / Umweltliche Größen / EPD EN 15804 / LCI Indikatoren",
          "nameClass": "GaBiCategories"
        }
      },
      {
        "id": "ILCDex:63a79af11ab0467745a808dc6fc9d4ca_exchanges_exchange_16",
        "dataSetInternalID": 15,
        "referenceToFlowDataSet": {
          "id": "ILCDex:63a79af11ab0467745a808dc6fc9d4ca_exchanges_exchange_16_referenceToFlowDataSet",
          "shortDescription": [
            {
              "id": "ILCDex:63a79af11ab0467745a808dc6fc9d4ca_exchanges_exchange_16_referenceToFlowDataSet_shortDescription_01",
              "value": "Materials for recycling (MFR)",
              "lang": "en"
            }
          ],
          "type": "flow data set",
          "refObjectId": "d7fe48a5-4103-49c8-9aae-b0b5dfdbd6ae"
        },
        "meanAmount": 0.0,
        "resolvedFlowVersion": "30.00.000",
        "flowProperties": [],
        "typeOfFlow": "Other flow",
        "exchangeDirection": "OUTPUT",
        "otherEx": {
          "id": "ILCDex:63a79af11ab0467745a808dc6fc9d4ca_exchanges_exchange_16_otherEx",
          "anies": [
            {
              "id": "ILCDex:63a79af11ab0467745a808dc6fc9d4ca_exchanges_exchange_16_otherEx_anies_moduleA1",
              "value": "13.9171550192986",
              "module": "A1"
            },
            {
              "id": "ILCDex:63a79af11ab0467745a808dc6fc9d4ca_exchanges_exchange_16_otherEx_anies_moduleA2",
              "value": "0",
              "module": "A2"
            },
            {
              "id": "ILCDex:63a79af11ab0467745a808dc6fc9d4ca_exchanges_exchange_16_otherEx_anies_moduleA3",
              "value": "38.59",
              "module": "A3"
            },
            {
              "id": "ILCDex:63a79af11ab0467745a808dc6fc9d4ca_exchanges_exchange_16_otherEx_anies_moduleA1A3",
              "value": "52.5071550192986",
              "module": "A1-A3"
            },
            {
              "id": "ILCDex:63a79af11ab0467745a808dc6fc9d4ca_exchanges_exchange_16_otherEx_anies_moduleA4",
              "value": "ND",
              "module": "A4"
            },
            {
              "id": "ILCDex:63a79af11ab0467745a808dc6fc9d4ca_exchanges_exchange_16_otherEx_anies_moduleA5",
              "value": "ND",
              "module": "A5"
            },
            {
              "id": "ILCDex:63a79af11ab0467745a808dc6fc9d4ca_exchanges_exchange_16_otherEx_anies_moduleB1",
              "value": "0",
              "module": "B1"
            },
            {
              "id": "ILCDex:63a79af11ab0467745a808dc6fc9d4ca_exchanges_exchange_16_otherEx_anies_moduleB2",
              "value": "0",
              "module": "B2"
            },
            {
              "id": "ILCDex:63a79af11ab0467745a808dc6fc9d4ca_exchanges_exchange_16_otherEx_anies_moduleB3",
              "value": "0",
              "module": "B3"
            },
            {
              "id": "ILCDex:63a79af11ab0467745a808dc6fc9d4ca_exchanges_exchange_16_otherEx_anies_moduleB4",
              "value": "0",
              "module": "B4"
            },
            {
              "id": "ILCDex:63a79af11ab0467745a808dc6fc9d4ca_exchanges_exchange_16_otherEx_anies_moduleB5",
              "value": "0",
              "module": "B5"
            },
            {
              "id": "ILCDex:63a79af11ab0467745a808dc6fc9d4ca_exchanges_exchange_16_otherEx_anies_moduleB6",
              "value": "0",
              "module": "B6"
            },
            {
              "id": "ILCDex:63a79af11ab0467745a808dc6fc9d4ca_exchanges_exchange_16_otherEx_anies_moduleB7",
              "value": "0",
              "module": "B7"
            },
            {
              "id": "ILCDex:63a79af11ab0467745a808dc6fc9d4ca_exchanges_exchange_16_otherEx_anies_moduleC1",
              "value": "0",
              "module": "C1"
            },
            {
              "id": "ILCDex:63a79af11ab0467745a808dc6fc9d4ca_exchanges_exchange_16_otherEx_anies_moduleC2",
              "value": "0",
              "module": "C2"
            },
            {
              "id": "ILCDex:63a79af11ab0467745a808dc6fc9d4ca_exchanges_exchange_16_otherEx_anies_moduleC3",
              "value": "1982.475",
              "module": "C3"
            },
            {
              "id": "ILCDex:63a79af11ab0467745a808dc6fc9d4ca_exchanges_exchange_16_otherEx_anies_moduleC4",
              "value": "0",
              "module": "C4"
            },
            {
              "id": "ILCDex:63a79af11ab0467745a808dc6fc9d4ca_exchanges_exchange_16_otherEx_anies_moduleD",
              "value": "0",
              "module": "D"
            },
            {
              "id": "ILCDex:63a79af11ab0467745a808dc6fc9d4ca_exchanges_exchange_16_otherEx_anies_19",
              "name": "referenceToUnitGroupDataSet",
              "objectValue": {
                "id": "ILCDex:63a79af11ab0467745a808dc6fc9d4ca_exchanges_exchange_16_otherEx_anies_19_objectValue",
                "shortDescription": [
                  {
                    "id": "ILCDex:63a79af11ab0467745a808dc6fc9d4ca_exchanges_exchange_16_otherEx_anies_19_objectValue_shortDescription_01",
                    "value": "kg"
                  }
                ],
                "type": "unit group data set",
                "refObjectId": "ad38d542-3fe9-439d-9b95-2f5f7752acaf",
                "refObjectUri": "../unitgroups/ad38d542-3fe9-439d-9b95-2f5f7752acaf"
              }
            }
          ]
        },
        "classificationEx": {
          "id": "ILCDex:63a79af11ab0467745a808dc6fc9d4ca_exchanges_exchange_16_classificationEx",
          "classHierarchy": "Größen / Umweltliche Größen / EPD EN 15804 / LCI Indikatoren",
          "nameClass": "GaBiCategories"
        }
      },
      {
        "id": "ILCDex:63a79af11ab0467745a808dc6fc9d4ca_exchanges_exchange_17",
        "dataSetInternalID": 16,
        "referenceToFlowDataSet": {
          "id": "ILCDex:63a79af11ab0467745a808dc6fc9d4ca_exchanges_exchange_17_referenceToFlowDataSet",
          "shortDescription": [
            {
              "id": "ILCDex:63a79af11ab0467745a808dc6fc9d4ca_exchanges_exchange_17_referenceToFlowDataSet_shortDescription_01",
              "value": "Materials for energy recovery (MER)",
              "lang": "en"
            }
          ],
          "type": "flow data set",
          "refObjectId": "59a9181c-3aaf-46ee-8b13-2b3723b6e447"
        },
        "meanAmount": 0.0,
        "resolvedFlowVersion": "30.00.000",
        "flowProperties": [],
        "typeOfFlow": "Other flow",
        "exchangeDirection": "OUTPUT",
        "otherEx": {
          "id": "ILCDex:63a79af11ab0467745a808dc6fc9d4ca_exchanges_exchange_17_otherEx",
          "anies": [
            {
              "id": "ILCDex:63a79af11ab0467745a808dc6fc9d4ca_exchanges_exchange_17_otherEx_anies_moduleA1",
              "value": "0",
              "module": "A1"
            },
            {
              "id": "ILCDex:63a79af11ab0467745a808dc6fc9d4ca_exchanges_exchange_17_otherEx_anies_moduleA2",
              "value": "0",
              "module": "A2"
            },
            {
              "id": "ILCDex:63a79af11ab0467745a808dc6fc9d4ca_exchanges_exchange_17_otherEx_anies_moduleA3",
              "value": "0",
              "module": "A3"
            },
            {
              "id": "ILCDex:63a79af11ab0467745a808dc6fc9d4ca_exchanges_exchange_17_otherEx_anies_moduleA1A3",
              "value": "0",
              "module": "A1-A3"
            },
            {
              "id": "ILCDex:63a79af11ab0467745a808dc6fc9d4ca_exchanges_exchange_17_otherEx_anies_moduleA4",
              "value": "ND",
              "module": "A4"
            },
            {
              "id": "ILCDex:63a79af11ab0467745a808dc6fc9d4ca_exchanges_exchange_17_otherEx_anies_moduleA5",
              "value": "ND",
              "module": "A5"
            },
            {
              "id": "ILCDex:63a79af11ab0467745a808dc6fc9d4ca_exchanges_exchange_17_otherEx_anies_moduleB1",
              "value": "0",
              "module": "B1"
            },
            {
              "id": "ILCDex:63a79af11ab0467745a808dc6fc9d4ca_exchanges_exchange_17_otherEx_anies_moduleB2",
              "value": "0",
              "module": "B2"
            },
            {
              "id": "ILCDex:63a79af11ab0467745a808dc6fc9d4ca_exchanges_exchange_17_otherEx_anies_moduleB3",
              "value": "0",
              "module": "B3"
            },
            {
              "id": "ILCDex:63a79af11ab0467745a808dc6fc9d4ca_exchanges_exchange_17_otherEx_anies_moduleB4",
              "value": "0",
              "module": "B4"
            },
            {
              "id": "ILCDex:63a79af11ab0467745a808dc6fc9d4ca_exchanges_exchange_17_otherEx_anies_moduleB5",
              "value": "0",
              "module": "B5"
            },
            {
              "id": "ILCDex:63a79af11ab0467745a808dc6fc9d4ca_exchanges_exchange_17_otherEx_anies_moduleB6",
              "value": "0",
              "module": "B6"
            },
            {
              "id": "ILCDex:63a79af11ab0467745a808dc6fc9d4ca_exchanges_exchange_17_otherEx_anies_moduleB7",
              "value": "0",
              "module": "B7"
            },
            {
              "id": "ILCDex:63a79af11ab0467745a808dc6fc9d4ca_exchanges_exchange_17_otherEx_anies_moduleC1",
              "value": "0",
              "module": "C1"
            },
            {
              "id": "ILCDex:63a79af11ab0467745a808dc6fc9d4ca_exchanges_exchange_17_otherEx_anies_moduleC2",
              "value": "0",
              "module": "C2"
            },
            {
              "id": "ILCDex:63a79af11ab0467745a808dc6fc9d4ca_exchanges_exchange_17_otherEx_anies_moduleC3",
              "value": "0",
              "module": "C3"
            },
            {
              "id": "ILCDex:63a79af11ab0467745a808dc6fc9d4ca_exchanges_exchange_17_otherEx_anies_moduleC4",
              "value": "0",
              "module": "C4"
            },
            {
              "id": "ILCDex:63a79af11ab0467745a808dc6fc9d4ca_exchanges_exchange_17_otherEx_anies_moduleD",
              "value": "0",
              "module": "D"
            },
            {
              "id": "ILCDex:63a79af11ab0467745a808dc6fc9d4ca_exchanges_exchange_17_otherEx_anies_19",
              "name": "referenceToUnitGroupDataSet",
              "objectValue": {
                "id": "ILCDex:63a79af11ab0467745a808dc6fc9d4ca_exchanges_exchange_17_otherEx_anies_19_objectValue",
                "shortDescription": [
                  {
                    "id": "ILCDex:63a79af11ab0467745a808dc6fc9d4ca_exchanges_exchange_17_otherEx_anies_19_objectValue_shortDescription_01",
                    "value": "kg"
                  }
                ],
                "type": "unit group data set",
                "refObjectId": "ad38d542-3fe9-439d-9b95-2f5f7752acaf",
                "refObjectUri": "../unitgroups/ad38d542-3fe9-439d-9b95-2f5f7752acaf"
              }
            }
          ]
        },
        "classificationEx": {
          "id": "ILCDex:63a79af11ab0467745a808dc6fc9d4ca_exchanges_exchange_17_classificationEx",
          "classHierarchy": "Größen / Umweltliche Größen / EPD EN 15804 / LCI Indikatoren",
          "nameClass": "GaBiCategories"
        }
      },
      {
        "id": "ILCDex:63a79af11ab0467745a808dc6fc9d4ca_exchanges_exchange_18",
        "dataSetInternalID": 17,
        "referenceToFlowDataSet": {
          "id": "ILCDex:63a79af11ab0467745a808dc6fc9d4ca_exchanges_exchange_18_referenceToFlowDataSet",
          "shortDescription": [
            {
              "id": "ILCDex:63a79af11ab0467745a808dc6fc9d4ca_exchanges_exchange_18_referenceToFlowDataSet_shortDescription_01",
              "value": "Exported electrical energy (EEE)",
              "lang": "en"
            }
          ],
          "type": "flow data set",
          "refObjectId": "4da0c987-2b76-40d6-9e9e-82a017aaaf29"
        },
        "meanAmount": 0.0,
        "resolvedFlowVersion": "35.00.000",
        "flowProperties": [],
        "typeOfFlow": "Other flow",
        "exchangeDirection": "OUTPUT",
        "otherEx": {
          "id": "ILCDex:63a79af11ab0467745a808dc6fc9d4ca_exchanges_exchange_18_otherEx",
          "anies": [
            {
              "id": "ILCDex:63a79af11ab0467745a808dc6fc9d4ca_exchanges_exchange_18_otherEx_anies_moduleA1",
              "value": "0",
              "module": "A1"
            },
            {
              "id": "ILCDex:63a79af11ab0467745a808dc6fc9d4ca_exchanges_exchange_18_otherEx_anies_moduleA2",
              "value": "0",
              "module": "A2"
            },
            {
              "id": "ILCDex:63a79af11ab0467745a808dc6fc9d4ca_exchanges_exchange_18_otherEx_anies_moduleA3",
              "value": "0",
              "module": "A3"
            },
            {
              "id": "ILCDex:63a79af11ab0467745a808dc6fc9d4ca_exchanges_exchange_18_otherEx_anies_moduleA1A3",
              "value": "0",
              "module": "A1-A3"
            },
            {
              "id": "ILCDex:63a79af11ab0467745a808dc6fc9d4ca_exchanges_exchange_18_otherEx_anies_moduleA4",
              "value": "ND",
              "module": "A4"
            },
            {
              "id": "ILCDex:63a79af11ab0467745a808dc6fc9d4ca_exchanges_exchange_18_otherEx_anies_moduleA5",
              "value": "ND",
              "module": "A5"
            },
            {
              "id": "ILCDex:63a79af11ab0467745a808dc6fc9d4ca_exchanges_exchange_18_otherEx_anies_moduleB1",
              "value": "0",
              "module": "B1"
            },
            {
              "id": "ILCDex:63a79af11ab0467745a808dc6fc9d4ca_exchanges_exchange_18_otherEx_anies_moduleB2",
              "value": "0",
              "module": "B2"
            },
            {
              "id": "ILCDex:63a79af11ab0467745a808dc6fc9d4ca_exchanges_exchange_18_otherEx_anies_moduleB3",
              "value": "0",
              "module": "B3"
            },
            {
              "id": "ILCDex:63a79af11ab0467745a808dc6fc9d4ca_exchanges_exchange_18_otherEx_anies_moduleB4",
              "value": "0",
              "module": "B4"
            },
            {
              "id": "ILCDex:63a79af11ab0467745a808dc6fc9d4ca_exchanges_exchange_18_otherEx_anies_moduleB5",
              "value": "0",
              "module": "B5"
            },
            {
              "id": "ILCDex:63a79af11ab0467745a808dc6fc9d4ca_exchanges_exchange_18_otherEx_anies_moduleB6",
              "value": "0",
              "module": "B6"
            },
            {
              "id": "ILCDex:63a79af11ab0467745a808dc6fc9d4ca_exchanges_exchange_18_otherEx_anies_moduleB7",
              "value": "0",
              "module": "B7"
            },
            {
              "id": "ILCDex:63a79af11ab0467745a808dc6fc9d4ca_exchanges_exchange_18_otherEx_anies_moduleC1",
              "value": "0",
              "module": "C1"
            },
            {
              "id": "ILCDex:63a79af11ab0467745a808dc6fc9d4ca_exchanges_exchange_18_otherEx_anies_moduleC2",
              "value": "0",
              "module": "C2"
            },
            {
              "id": "ILCDex:63a79af11ab0467745a808dc6fc9d4ca_exchanges_exchange_18_otherEx_anies_moduleC3",
              "value": "0",
              "module": "C3"
            },
            {
              "id": "ILCDex:63a79af11ab0467745a808dc6fc9d4ca_exchanges_exchange_18_otherEx_anies_moduleC4",
              "value": "0",
              "module": "C4"
            },
            {
              "id": "ILCDex:63a79af11ab0467745a808dc6fc9d4ca_exchanges_exchange_18_otherEx_anies_moduleD",
              "value": "0",
              "module": "D"
            },
            {
              "id": "ILCDex:63a79af11ab0467745a808dc6fc9d4ca_exchanges_exchange_18_otherEx_anies_19",
              "name": "referenceToUnitGroupDataSet",
              "objectValue": {
                "id": "ILCDex:63a79af11ab0467745a808dc6fc9d4ca_exchanges_exchange_18_otherEx_anies_19_objectValue",
                "shortDescription": [
                  {
                    "id": "ILCDex:63a79af11ab0467745a808dc6fc9d4ca_exchanges_exchange_18_otherEx_anies_19_objectValue_shortDescription_01",
                    "value": "MJ"
                  }
                ],
                "type": "unit group data set",
                "refObjectId": "93a60a57-a3c8-11da-a746-0800200c9a66",
                "refObjectUri": "../unitgroups/93a60a57-a3c8-11da-a746-0800200c9a66"
              }
            }
          ]
        },
        "classificationEx": {
          "id": "ILCDex:63a79af11ab0467745a808dc6fc9d4ca_exchanges_exchange_18_classificationEx",
          "classHierarchy": "Quantities / Environmental quantities / EPD EN 15804 / LCI indicators",
          "nameClass": "GaBiCategories"
        }
      },
      {
        "id": "ILCDex:63a79af11ab0467745a808dc6fc9d4ca_exchanges_exchange_19",
        "dataSetInternalID": 18,
        "referenceToFlowDataSet": {
          "id": "ILCDex:63a79af11ab0467745a808dc6fc9d4ca_exchanges_exchange_19_referenceToFlowDataSet",
          "shortDescription": [
            {
              "id": "ILCDex:63a79af11ab0467745a808dc6fc9d4ca_exchanges_exchange_19_referenceToFlowDataSet_shortDescription_01",
              "value": "Exported thermal energy (EET)",
              "lang": "en"
            }
          ],
          "type": "flow data set",
          "refObjectId": "98daf38a-7a79-46d3-9a37-2b7bd0955810"
        },
        "meanAmount": 0.0,
        "resolvedFlowVersion": "35.00.000",
        "flowProperties": [],
        "typeOfFlow": "Other flow",
        "exchangeDirection": "OUTPUT",
        "otherEx": {
          "id": "ILCDex:63a79af11ab0467745a808dc6fc9d4ca_exchanges_exchange_19_otherEx",
          "anies": [
            {
              "id": "ILCDex:63a79af11ab0467745a808dc6fc9d4ca_exchanges_exchange_19_otherEx_anies_moduleA1",
              "value": "0",
              "module": "A1"
            },
            {
              "id": "ILCDex:63a79af11ab0467745a808dc6fc9d4ca_exchanges_exchange_19_otherEx_anies_moduleA2",
              "value": "0",
              "module": "A2"
            },
            {
              "id": "ILCDex:63a79af11ab0467745a808dc6fc9d4ca_exchanges_exchange_19_otherEx_anies_moduleA3",
              "value": "0",
              "module": "A3"
            },
            {
              "id": "ILCDex:63a79af11ab0467745a808dc6fc9d4ca_exchanges_exchange_19_otherEx_anies_moduleA1A3",
              "value": "0",
              "module": "A1-A3"
            },
            {
              "id": "ILCDex:63a79af11ab0467745a808dc6fc9d4ca_exchanges_exchange_19_otherEx_anies_moduleA4",
              "value": "ND",
              "module": "A4"
            },
            {
              "id": "ILCDex:63a79af11ab0467745a808dc6fc9d4ca_exchanges_exchange_19_otherEx_anies_moduleA5",
              "value": "ND",
              "module": "A5"
            },
            {
              "id": "ILCDex:63a79af11ab0467745a808dc6fc9d4ca_exchanges_exchange_19_otherEx_anies_moduleB1",
              "value": "0",
              "module": "B1"
            },
            {
              "id": "ILCDex:63a79af11ab0467745a808dc6fc9d4ca_exchanges_exchange_19_otherEx_anies_moduleB2",
              "value": "0",
              "module": "B2"
            },
            {
              "id": "ILCDex:63a79af11ab0467745a808dc6fc9d4ca_exchanges_exchange_19_otherEx_anies_moduleB3",
              "value": "0",
              "module": "B3"
            },
            {
              "id": "ILCDex:63a79af11ab0467745a808dc6fc9d4ca_exchanges_exchange_19_otherEx_anies_moduleB4",
              "value": "0",
              "module": "B4"
            },
            {
              "id": "ILCDex:63a79af11ab0467745a808dc6fc9d4ca_exchanges_exchange_19_otherEx_anies_moduleB5",
              "value": "0",
              "module": "B5"
            },
            {
              "id": "ILCDex:63a79af11ab0467745a808dc6fc9d4ca_exchanges_exchange_19_otherEx_anies_moduleB6",
              "value": "0",
              "module": "B6"
            },
            {
              "id": "ILCDex:63a79af11ab0467745a808dc6fc9d4ca_exchanges_exchange_19_otherEx_anies_moduleB7",
              "value": "0",
              "module": "B7"
            },
            {
              "id": "ILCDex:63a79af11ab0467745a808dc6fc9d4ca_exchanges_exchange_19_otherEx_anies_moduleC1",
              "value": "0",
              "module": "C1"
            },
            {
              "id": "ILCDex:63a79af11ab0467745a808dc6fc9d4ca_exchanges_exchange_19_otherEx_anies_moduleC2",
              "value": "0",
              "module": "C2"
            },
            {
              "id": "ILCDex:63a79af11ab0467745a808dc6fc9d4ca_exchanges_exchange_19_otherEx_anies_moduleC3",
              "value": "0",
              "module": "C3"
            },
            {
              "id": "ILCDex:63a79af11ab0467745a808dc6fc9d4ca_exchanges_exchange_19_otherEx_anies_moduleC4",
              "value": "0",
              "module": "C4"
            },
            {
              "id": "ILCDex:63a79af11ab0467745a808dc6fc9d4ca_exchanges_exchange_19_otherEx_anies_moduleD",
              "value": "0",
              "module": "D"
            },
            {
              "id": "ILCDex:63a79af11ab0467745a808dc6fc9d4ca_exchanges_exchange_19_otherEx_anies_19",
              "name": "referenceToUnitGroupDataSet",
              "objectValue": {
                "id": "ILCDex:63a79af11ab0467745a808dc6fc9d4ca_exchanges_exchange_19_otherEx_anies_19_objectValue",
                "shortDescription": [
                  {
                    "id": "ILCDex:63a79af11ab0467745a808dc6fc9d4ca_exchanges_exchange_19_otherEx_anies_19_objectValue_shortDescription_01",
                    "value": "MJ"
                  }
                ],
                "type": "unit group data set",
                "refObjectId": "93a60a57-a3c8-11da-a746-0800200c9a66",
                "refObjectUri": "../unitgroups/93a60a57-a3c8-11da-a746-0800200c9a66"
              }
            }
          ]
        },
        "classificationEx": {
          "id": "ILCDex:63a79af11ab0467745a808dc6fc9d4ca_exchanges_exchange_19_classificationEx",
          "classHierarchy": "Quantities / Environmental quantities / EPD EN 15804 / LCI indicators",
          "nameClass": "GaBiCategories"
        }
      }
    ]
  }
}
